the verification tool for CBS

ExBasic.v
@@ -14,11 +14,16 @@ Notice: readers should read Language.v first.
 
 Author: Bowen Zhang.
 
-Date : 2022.01.06
+Date : 2023.01.06
 *)
 
 From SLF (* TLC *) Require Export LibCore TLCbuffer.
-From SLF (* Sep *) Require Export Rules.
+From SLF (* Sep *) Require Export TripleAndRules.
+
+Notation "[ ]" := nil (format "[ ]") : liblist_scope.
+Notation "[ x ]" := (cons x nil)  : liblist_scope.
+Notation "[ x ; y ; .. ; z ]" :=  (cons x (cons y .. (cons z nil) ..)) : liblist_scope.
+
 
 (* ================================================================= *)
 (** Some ltac to simplify the verification *)
@@ -116,6 +121,13 @@ Ltac fix_rem :=
 
 (* ###########################  Examples #################################*)
 
+Lemma san : forall (P Q R:Prop),
+  (P -> Q) -> (Q -> R) -> P -> R.
+Proof.
+  intros P Q R. intros H1 H2 H3.
+  apply H2. apply H1. apply H3.
+Qed.
+
 (* !! Need to read the Language.v firstly !! *)
 Export NotationForTrm.
 Export NotationForVariables.
@@ -125,32 +137,112 @@ Open Scope trm_scope.
 Open Scope Z_scope.
 
 (*========================= Copy a block ================================*)
-(*
-val_fun bk 
-  (trm_let ln (trm_app (trm_val (val_bval bval_get)) (trm_var bk))
-	  trm_app (trm_val (val_bval bval_create)) (trm_var ln))
-*)
 
 Definition Copy_blk : val := 
-  Fun 'bk :=
-    Let 'ln := 'bget 'bk in
-    'bcreate 'ln.
+  Fun 'f 'n :=                       
+  	Let 'b := 'nthblk 'f 'n in  
+    Let 'ln := 'bget 'b in
+      'bcreate 'ln.
 
+(* Unoptimized coding forms *)
+Definition Copy_blk' : val := 
+Fun 'f 'n := (
+  Let 'b := trm_app
+              (trm_app (trm_val (val_fprim fprim_nthblk))
+                       (trm_var 'f)) (trm_var 'n) in
+  Let 'ln := trm_app (trm_val (val_bprim bprim_get)) (trm_var 'b) in
+  trm_app (trm_val (val_bprim bprim_create)) (trm_var 'ln)).
 
-Lemma triple_Copy_blk : forall Hf (bp:bloc) (l:listint),
-  triple (Copy_blk bp)
-    (\R[Hf, bp ~b~> l] )
-    (fun r => \exists bp',\[r=(val_bloc bp')] \* (\R[Hf,(bp' ~b~> l) \b* (bp ~b~> l)])).
+(* Consistent in both forms, our optimized codes are more readable *)
+Fact equiv_Copy: Copy_blk = Copy_blk'.
+Proof. reflexivity. Qed.
+
+(* the specification and proof of copy a block *)
+Lemma triple_Copy_blk : forall (f:floc) (b:bloc) (lb:list bloc) (ln:list int) (n:int),
+  triple (Copy_blk f n)
+    (\[b = (nth_default bnull (Z.to_nat n) lb)] \* (\R[f ~f~> lb, b ~b~> ln]) )
+    (fun r => \exists b1,\[r=(val_bloc b1)] \* (\R[f ~f~> lb,(b1 ~b~> ln) \b* (b ~b~> ln)])).
 Proof.
-  intros. applys* triple_app_fun.
+  intros. apply triple_hpure. intros ->.
+  eapply triple_app_fun2. reflexivity. auto. simpl.
+  eapply triple_let. apply triple_fget_nth_blk.
+  intros. simpl.
+  apply triple_hpure. intros ->.
   applys triple_let triple_bget. ext.
   applys triple_conseq_frame triple_bcreate.
   rewrite* hstar_hempty_l'.
   introv M. rewrite hstar_hexists in M.
-  destruct M as (bp'&M).
+  destruct M as (b1&M).
   rewrite hstar_assoc, hstar_sep, hfstar_hempty_l in M.
-  exists~ bp'.
+  exists~ b1.
 Qed.
+
+(* Another spec that directly takes pure fact as the premise *)
+Lemma triple_Copy_blk' : forall (f:floc) (b:bloc) (lb:list bloc) (ln:list int) (n:int),
+b = (nth_default bnull (Z.to_nat n) lb) ->
+  triple (Copy_blk f n)
+    (\R[f ~f~> lb, b ~b~> ln])
+    (fun r => \exists b1,\[r=(val_bloc b1)] \* (\R[f ~f~> lb,(b1 ~b~> ln) \b* (b ~b~> ln)])).
+Proof.
+  introv ->. applys* triple_app_fun2. ext.
+  applys triple_let triple_fget_nth_blk. ext.
+  applys triple_let triple_bget. ext.
+  applys triple_conseq_frame triple_bcreate.
+  rewrite* hstar_hempty_l'.
+  introv M. rewrite hstar_hexists in M.
+  destruct M as (b1&M).
+  rewrite hstar_assoc, hstar_sep, hfstar_hempty_l in M.
+  exists~ b1.
+Qed.
+
+(* Notice: the 1st spec can be directly proved by the 2nd one *)
+Lemma triple_Copy_blk'' : forall (f:floc) (b:bloc) (lb:list bloc) (ln:list int) (n:int),
+  triple (Copy_blk f n)
+    (\[b = (nth_default bnull (Z.to_nat n) lb)] \* (\R[f ~f~> lb, b ~b~> ln]) )
+    (fun r => \exists b1,\[r=(val_bloc b1)] \* (\R[f ~f~> lb,(b1 ~b~> ln) \b* (b ~b~> ln)])).
+Proof. ext. applys* triple_Copy_blk'. Qed.
+
+
+
+(*========================= Move a block ================================*)
+Definition Move_blk :=
+  Fun 'f 'i :=
+    Let 'b := 'nthblk 'f 'i in
+    Let 'b1 := Copy_blk 'f 'i in
+    'set 'f 'i 'as 'b1 ';
+    'bdelete 'b.
+
+Lemma triple_Move_blk : forall (f:floc) (b:bloc) (lb:list bloc) (ln:list int) (n:int),
+b = (nth_default bnull (Z.to_nat n) lb) ->
+  triple (Move_blk f n)
+    (\R[ f ~f~> lb, b ~b~> ln ])
+    (fun _ => \exists b',
+              (\R[( f ~f~> (LibList.update (to_nat n) b' lb)),(b' ~b~> ln)])).
+Proof.
+  introv ->.
+  applys* triple_app_fun2. simpls.
+  applys triple_let triple_fget_nth_blk. ext.
+  applys* triple_let triple_Copy_blk'.
+  ext. intros b'. ext.
+  applys triple_seq.
+  apply triple_fset_nth_blk.
+  applys triple_conseq_frame triple_bdelete.
+  rewrite hstar_sep, hfstar_hempty_r, hbstar_comm.
+  applys himpl_refl.
+  intros r. rewrite hstar_sep, hfstar_hempty_r, hbstar_hempty_l.
+  intros h (MA&MB).
+  exists b'. splits~.
+Qed.
+
+(* Set Printing Coercions.
+	Print Copy_fblk .
+	Unset Printing Coercions.
+
+Instance Inhab_listint : Inhab (list int).
+Proof using. apply (Inhab_of_val (0::nil) ). Qed.
+
+Instance Inhab_listbloc : Inhab (list bloc).
+Proof using. apply (Inhab_of_val (bnull::nil) ). Qed. *)
 
 (*========================= Remove a file (rec) ================================*)
 (*   --pseudo code--
@@ -172,14 +264,14 @@ Definition Remove_f :=
     If_ 'be
     Then ('fdelete 'f)
     Else
-      Let 'bk := 'nth_blk 'f 'i in
+      Let 'bk := 'nthblk 'f 'i in
       Let 'i1 := 'i '+ 1 in
       'bdelete 'bk ';
       'F 'f 'i1.
 
-Lemma triple_Remove_f:  forall Hf Hb (f:floc) (p1 p2 p3 p4:bloc) (l1 l2 l3 l4:listint),
-  Hf = ( f ~f~> (p1::p2::p3::p4::nil) ) ->
-  Hb = ( (p1 ~b~> l1) \b* (p2 ~b~> l2) \b* (p3 ~b~> l3) \b* (p4 ~b~> l4) ) ->
+Lemma triple_Remove_f:  forall Hf Hb (f:floc) (b1 b2 b3 b4:bloc) (lb1 lb2 lb3 lb4:list int),
+  Hf = ( f ~f~> (b1::b2::b3::b4::nil) ) ->
+  Hb = ( (b1 ~b~> lb1) \b* (b2 ~b~> lb2) \b* (b3 ~b~> lb3) \b* (b4 ~b~> lb4) ) ->
   triple (Remove_f f 0)
     (\R[Hf,Hb])
     (fun _ =>  \R[\f[],\b[]]).
@@ -193,25 +285,25 @@ Qed.
 
 
 (*========================= Read a file (rec) ================================*)
-Definition Read_f := 
+Definition ReadFile := 
   Fix 'F 'f 'i :=
     Let 'n := 'fsize 'f in
     Let 'be := ('i '= 'n) in
     If_ 'be
     Then (val_listint nil)
     Else
-      Let 'bk := 'nth_blk 'f 'i in
+      Let 'bk := 'nthblk 'f 'i in
       Let 'i1 := 'i '+ 1 in
       Let 'ln := 'bget 'bk in
       Let 'ln1 := 'F 'f 'i1 in
       'ln '++ 'ln1.
 
-Lemma triple_Read_f: forall Hf Hb (f:floc) (p1 p2 p3:bloc) (n1 n2 n3 n4 n5:int),
-  Hf = ( f ~f~> (p1::p2::p3::nil) ) ->
-  Hb = ( (p1 ~b~> (n1::n2::nil)) \b* (p2 ~b~> (n3::n4::nil)) \b* (p3 ~b~> (n5::nil)) ) ->
-  triple (Read_f f 0)
+Lemma triple_ReadFile: forall Hf Hb (f:floc) (b1 b2 b3:bloc) (n1 n2 n3 n4 n5:int),
+  Hf = ( f ~f~> (b1::b2::b3::nil) ) ->
+  Hb = ( (b1 ~b~> (n1::n2::nil)) \b* (b2 ~b~> (n3::n4::nil)) \b* (b3 ~b~> (n5::nil)) ) ->
+  triple (ReadFile f 0)
     (\R[Hf,Hb])
-    (fun r => \[r= val_listint (n1::n2::n3::n4::n5::nil)] \* \R[Hf,Hb]).
+    (fun r => \[r= val_listint (n1::n2::n3::n4::n5::nil) ] \* \R[Hf,Hb]).
 Proof.
   fix_read.
   rewrite hstar_sep, hfstar_hempty_l. apply himpl_refl.
@@ -238,21 +330,126 @@ Proof.
   rewrite hbstar_comm,hbstar_assoc. apply himpl_refl.
 Qed.
 
-(*===================== Create files ===========================*)
 
-(*-------- create a file with two blocks -----------*)
+Ltac exp_fix_create :=
+  applys* triple_app_fix2;
+  applys triple_let triple_list_len; ext;
+  applys triple_let triple_le; ext;
+  applys triple_if; case_if*;
+  applys triple_let triple_list_hd_bk; ext;
+  applys triple_let triple_list_tl_bk; ext;
+  applys triple_let.
+
+Ltac cre_pre :=
+  rewrite hstar_sep; rewrite hfstar_hempty_r, hbstar_hempty_l;
+  apply himpl_refl.
+
+Ltac cre_ext:=
+intros r; simpl; rewrite hstar_hexists;
+  applys triple_hexists.
+
+Ltac cre_exp_fix:=
+  intros; applys* triple_app_fix2;
+  applys triple_let triple_list_len;
+  ext; applys triple_let triple_le; ext;
+  applys triple_if; case_if*.
+
+(*===================== Create files ===========================*)
+Definition CreateBlks : val :=
+  Fix 'F 'l 'lb:=
+    Let 'm := 'len 'l in
+    Let 'be := ('m '<= 2) in
+    If_ 'be
+    Then 
+      Let 'bk := 'bcreate 'l in
+        'bk 'b+ 'lb
+    Else
+      Let 'l1 := 'hdblk 'l in
+      Let 'l2 := 'tlblk 'l in
+      Let 'bk1 := 'bcreate 'l1 in
+      Let 'lb1 := 'bk1 'b+ 'lb in
+        'F 'l2 'lb1.
+
+Lemma triple_CreateBlks : forall Hf (n1 n2 n3 n4 n5:int),
+  triple (CreateBlks (val_listint (n1::n2::n3::n4::n5::nil)) (val_listbloc nil))
+    (\R[Hf, \b[] ])
+     (fun r => \exists b1 b2 b3,( \[r=(val_listbloc (b3::b2::b1::nil))] \* 
+               (\R[Hf, (b1 ~b~> (n1::n2::nil)) \b* (b2 ~b~> (n3::n4::nil) \b* (b3 ~b~> (n5::nil)))]))).
+Proof.
+  cre_exp_fix. destruct C. auto.
+  applys triple_let triple_list_hd_bk. ext.
+  applys triple_let triple_list_tl_bk. ext.
+  applys triple_let.
+  applys triple_conseq_frame triple_bcreate.
+  cre_pre. intros r. apply himpl_refl.
+  cre_ext. intros b1.
+  rewrite hstar_hempty_r. ext.
+  applys triple_let triple_blist_buffer. ext.
+
+  exp_fix_create.
+  applys triple_conseq_frame triple_bcreate.
+  cre_pre. intros r. apply himpl_refl.
+  cre_ext. intros b2.
+  rewrite hstar_assoc, hstar_sep, hfstar_hempty_r. ext.
+  applys triple_let triple_blist_buffer. ext.
+
+  cre_exp_fix. applys triple_let.
+  applys triple_conseq_frame triple_bcreate.
+  rewrite hstar_sep, hfstar_hempty_r, hbstar_hempty_l. apply himpl_refl.
+  intros* r. apply himpl_refl. cre_ext. intros b3.
+  rewrite hstar_assoc, hstar_sep, hfstar_hempty_r. ext.
+  applys triple_conseq_frame triple_blist_buffer.
+  rewrite hstar_hempty_l'. apply himpl_refl.
+  intros r. rewrite hstar_hempty_r, hbstar_comm3.
+  intros h H. apply hstar_hpure_iff in H as (H1&H2).
+  exists b1 b2 b3.
+  applys hstar_hpure_iff. splits~.
+  destruct C1. rew_list. discriminate.
+Qed.
+
+Definition Create_File : val :=
+  Fun 'l:=
+    Let 'lb1 := CreateBlks 'l (val_listbloc nil) in
+    Let 'lb := 'frev 'lb1 in
+      'fcreate 'lb.
+
+
+Lemma triple_Create_File : forall (n1 n2 n3 n4 n5:int),
+  triple (Create_File (val_listint (n1::n2::n3::n4::n5::nil)) )
+    (\R[\f[], \b[] ])
+     (fun r => \exists f b1 b2 b3,( \[r= (val_floc f)] \* 
+               (\R[(f ~f~> (b1::b2::b3::nil)), (b1 ~b~> (n1::n2::nil)) \b* (b2 ~b~> (n3::n4::nil) \b* (b3 ~b~> (n5::nil)))]))).
+Proof.
+  intros. applys* triple_app_fun.
+  applys triple_let triple_CreateBlks.
+  intros v. ext. intros b1. ext. intros b2. ext. intros b3. ext.
+  applys triple_let.
+  applys triple_conseq_frame triple_blist_rev.
+  rewrite hstar_hempty_l'. apply himpl_refl.
+  intros r. rewrite hstar_assoc, hstar_hempty_l. apply himpl_refl.
+  ext.
+  applys triple_conseq_frame triple_fcreate.
+  rewrite hstar_hempty_r'. apply himpl_refl.
+  intros v. rewrite hstar_hempty_r'.
+  apply himpl_hexists_l. intros f.
+  intros h M. exists~ f b1 b2 b3.
+Qed.
+
+
+(*---------Other methods of creating files (not very smart)------*)
+(*--- create a file with two blocks ---*)
 Definition Create_blk2 : val :=
   Fun 'ln1 'ln2 :=
     Let 'bk1 := 'bcreate 'ln1 in
     Let 'bk2 := 'bcreate 'ln2 in
-    Let 'lb := 'fbuffer 'bk2 in
+    Let 'lb := 'buffer 'bk2 in
     'bk1 'b+ 'lb.
 
-Lemma triple_Create_blk2 : forall Hf (l1 l2:listint),
-  triple (Create_blk2 (val_listint l1) (val_listint l2))
+Lemma triple_Create_blk2 : forall Hf (ln1 ln2:list int),
+  triple (Create_blk2 (val_listint ln1) (val_listint ln2))
     (\R[Hf, \b[] ])
-     (fun r => \exists bp1 bp2,( \[r=(val_listbloc (bp1::bp2::nil))] \* 
-               (\R[Hf, (bp1 ~b~> l1) \b* (bp2 ~b~> l2)]))).
+     (fun r => \exists b1 b2,( \[r=(val_listbloc (b1::b2::nil))] \* 
+               (\R[Hf, (b1 ~b~> ln1) \b* (b2 ~b~> ln2)]))).
 Proof.
   intros. applys triple_app_fun2. reflexivity. auto.
   simpl. applys triple_let triple_bcreate'.
@@ -263,8 +460,8 @@ Proof.
   rewrite hstar_hempty_l'. apply himpl_refl.
   intros v. inner_femp.
   ext. intros b2. rewrite hbstar_assoc. ext.
-  applys triple_let triple_fbuffer. ext.
-  applys triple_conseq_frame triple_fbuffer_list.
+  applys triple_let triple_new_buffer. ext.
+  applys triple_conseq_frame triple_blist_buffer.
   outer_emp.
   { intros r h. rewrite hstar_hempty_r', hstar_hpure, hbstar_comm.
     intros (MA&MB). exists~ b1 b2. rewrite hstar_hpure. splits~. }
@@ -275,21 +472,19 @@ Definition Newf_blk2 :val :=
     Let 'lb := Create_blk2 'ln1 'ln2 in
     'fcreate 'lb.
 
-Lemma triple_Newb_con2 : forall (l1 l2:listint),
-  triple (Newf_blk2 (val_listint l1) (val_listint l2))
+Lemma triple_Newb_con2 : forall (ln1 ln2:list int),
+  triple (Newf_blk2 (val_listint ln1) (val_listint ln2))
     (\R[\f[], \b[] ])
-    (fun r => \exists bp1 bp2,
-      (\exists fp : floc,\[r = fp] \*
-        (\R[ fp ~f~> (bp1 :: bp2 :: nil),bp1 ~b~> l1 \b* bp2 ~b~> l2]))).
+    (fun r => \exists b1 b2,
+      (\exists f : floc,\[r = f] \*
+        (\R[ f ~f~> (b1 :: b2 :: nil),b1 ~b~> ln1 \b* b2 ~b~> ln2]))).
 Proof.
   intros. applys* triple_app_fun2.
   simpl. applys triple_let triple_Create_blk2.
-  intros v. ext. intros bp1. ext. intros bp2. ext.
+  intros v. ext. intros b1. ext. intros b2. ext.
   applys triple_conseq_frame triple_fcreate.
-  rewrite hstar_hempty_r'.
-  apply himpl_noduplicate2.
-  intros r. rewrite hstar_hempty_r.
-  intros h M. exists~ bp1 bp2.
+  rewrite hstar_hempty_r'. apply himpl_refl.
+  intros h M. rewrite hstar_hempty_r'. exists~ b1 b2.
 Qed.
 
 
@@ -301,24 +496,24 @@ Definition Create_blk3 : val :=
     Let 'lb1 := 'bk 'b+ 'lb in
     'frev 'lb1.
 
-Lemma triple_Create_blk3 : forall Hf (l1 l2 l3:listint),
-  triple (Create_blk3 (val_listint l1) (val_listint l2) (val_listint l3))
+Lemma triple_Create_blk3 : forall Hf (ln1 ln2 ln3:list int),
+  triple (Create_blk3 (val_listint ln1) (val_listint ln2) (val_listint ln3))
     (\R[Hf, \b[] ])
-    (fun r => \exists p1 p2 p3, \[r = val_listbloc (rev (p3 :: p2 :: p1 :: nil))] \*
-              (\R[ Hf, (p1 ~b~> l1 \b* p2 ~b~> l2 \b* p3 ~b~> l3)])).
+    (fun r => \exists b1 b2 b3, \[r = val_listbloc (rev (b3 :: b2 :: b1 :: nil))] \*
+              (\R[ Hf, (b1 ~b~> ln1 \b* b2 ~b~> ln2 \b* b3 ~b~> ln3)])).
 Proof.
   intros. applys* triple_app_fun3. simpl.
   applys triple_let triple_Create_blk2.
-  ext. intros bp2. ext. intros bp1. ext.
+  ext. intros b2. ext. intros b1. ext.
   applys triple_let.
   applys triple_conseq_frame triple_bcreate'.
   outer_emp. inner_femp.
-  ext. intros bp3. rewrite hbstar_assoc. ext.
-  applys triple_let triple_fbuffer_list. ext.
-  applys triple_conseq_frame triple_frev_blist.
+  ext. intros b3. rewrite hbstar_assoc. ext.
+  applys triple_let triple_blist_buffer. ext.
+  applys triple_conseq_frame triple_blist_rev.
   outer_emp.
   { intros r h. rewrite hstar_hempty_r', hstar_hpure, hbstar_comm3.
-    intros (MA&MB). exists~ bp1 bp2 bp3. rewrite hstar_hpure. splits~. }
+    intros (MA&MB). exists~ b1 b2 b3. rewrite hstar_hpure. splits~. }
 Qed.
 
 Definition Newf_blk3 :val := 
@@ -326,30 +521,50 @@ Definition Newf_blk3 :val :=
     Let 'lb := Create_blk3 'ln1 'ln2 'ln3 in
     'fcreate 'lb.
 
-Lemma triple_Newf_blk3 : forall (l1 l2 l3:listint),
-  triple (Newf_blk3 (val_listint l1) (val_listint l2) (val_listint l3))
+Lemma triple_Newf_blk3 : forall (ln1 ln2 ln3:list int),
+  triple (Newf_blk3 (val_listint ln1) (val_listint ln2) (val_listint ln3))
     (\R[\f[], \b[] ])
-    (fun r => \exists bp1 bp2 bp3,
+    (fun r => \exists b1 b2 b3,
       (\exists fp : floc, \[r = fp] \*
-        (\R[ fp ~f~> rev (bp3 :: bp2 :: bp1 :: nil),
-           bp1 ~b~> l1 \b* bp2 ~b~> l2 \b* bp3 ~b~> l3]))).
+        (\R[ fp ~f~> rev (b3 :: b2 :: b1 :: nil),
+           b1 ~b~> ln1 \b* b2 ~b~> ln2 \b* b3 ~b~> ln3]))).
 Proof.
   intros. applys triple_app_fun3.
   reflexivity. auto.
   simpl. applys triple_let.
   applys triple_Create_blk3.
-  ext. intros bp1. ext. intros bp2. ext. intros bp3. ext.
+  ext. intros b1. ext. intros b2. ext. intros b3. ext.
   applys triple_conseq_frame triple_fcreate.
-  rewrite hstar_hempty_r'.
-  apply himpl_noduplicate3.
-  intros v. rewrite hstar_hempty_r'.
-  intros h M. exists~ bp1 bp2 bp3.
+  rewrite hstar_hempty_r'. apply himpl_refl. 
+  intros h M. rewrite hstar_hempty_r'. exists~ b1 b2 b3.
 Qed.
 
 
 (*===================== Copy a file ===========================*)
 (*Copy the entire file, starting with the i-th block
   and storing the new block location list in the buffer*)
+
+(* copy a block directly from block tier *)
+Definition Copy_blk_dir : val := 
+  Fun 'bk :=
+    Let 'ln := 'bget 'bk in
+    'bcreate 'ln.
+
+Lemma triple_Copy_blk_dir : forall Hf (b:bloc) (l:list int),
+  triple (Copy_blk_dir b)
+    (\R[Hf, b ~b~> l] )
+    (fun r => \exists b',\[r=(val_bloc b')] \* (\R[Hf,(b' ~b~> l) \b* (b ~b~> l)])).
+Proof.
+  intros. applys* triple_app_fun.
+  applys triple_let triple_bget. ext.
+  applys triple_conseq_frame triple_bcreate.
+  rewrite* hstar_hempty_l'.
+  introv M. rewrite hstar_hexists in M.
+  destruct M as (b'&M).
+  rewrite hstar_assoc, hstar_sep, hfstar_hempty_l in M.
+  exists~ b'.
+Qed.
+
 Definition Copy_f_buffer := 
   Fix 'F 'f 'i :=
     Let 'n := 'fsize 'f in
@@ -357,26 +572,26 @@ Definition Copy_f_buffer :=
     If_ 'be
     Then (val_listbloc nil)
     Else
-      Let 'bk1 := 'nth_blk 'f 'i in
+      Let 'bk1 := 'nthblk 'f 'i in
       Let 'i := 'i '+ 1 in
-      Let 'bk := (Copy_blk 'bk1) in 
+      Let 'bk := (Copy_blk_dir 'bk1) in 
       Let 'lb := 'F 'f 'i in
       'bk 'b+ 'lb .
  
-Lemma triple_Copy_f_buffer:  forall f1 p1 ln,
+Lemma triple_Copy_f_buffer:  forall f1 b1 ln,
   triple (Copy_f_buffer (val_floc f1) 0)
-    (\R[f1 ~f~> (p1::nil),(p1 ~b~> ln)])
-    (fun r => \exists p1', \[r = val_listbloc (p1' :: nil)] \* 
-              \R[f1 ~f~> (p1::nil), ((p1' ~b~> ln) \b* (p1 ~b~> ln))]).
+    (\R[f1 ~f~> (b1::nil),(b1 ~b~> ln)])
+    (fun r => \exists b1', \[r = val_listbloc (b1' :: nil)] \* 
+              \R[f1 ~f~> (b1::nil), ((b1' ~b~> ln) \b* (b1 ~b~> ln))]).
 Proof.
   exp_fix. fix_body.
-  applys triple_let triple_Copy_blk.
+  applys triple_let triple_Copy_blk_dir.
   ext. intros bp1. ext.
   applys triple_let. 
   
   exp_fix.
   applys triple_val'. ext.
-  applys triple_conseq_frame triple_fbuffer_list.
+  applys triple_conseq_frame triple_blist_buffer.
   outer_emp.
   intros r. rewrite hstar_hempty_r'.
   intros h M. exists~ bp1.
@@ -398,10 +613,7 @@ Proof.
   applys triple_let triple_Copy_f_buffer.
   ext. intros p1'. ext.
   applys triple_conseq_frame triple_fcreate.
-  rewrite hstar_sep. intros h (MA&MB). split.
-  rewrite hfstar_hpure. split.
-  apply noduplicates_one. apply MA.
-  apply MB.
+  rewrite hstar_sep, hfstar_hempty_l. apply himpl_refl.
   intros r. intros h M.
   rewrite hstar_hexists in M.
   destruct M as (f2&M).
@@ -409,4 +621,32 @@ Proof.
   destruct M as (MA&MB).
   rewrite hstar_sep in MB.
   exists f2 p1'. rewrite hstar_hpure. splits~.
+Qed.
+
+Definition CopyFile :=
+  Fun 'f :=
+    Let 'ln := ReadFile 'f 0 in
+      Create_File 'ln.
+
+Ltac ext_blk :=
+rewrite hstar_hexists; apply himpl_hexists_l.
+
+Lemma triple_CopyFile: forall Hf Hb (f:floc) (b1 b2 b3:bloc) (n1 n2 n3 n4 n5:int),
+  Hf = ( f ~f~> (b1::b2::b3::nil) ) ->
+  Hb = ( (b1 ~b~> (n1::n2::nil)) \b* (b2 ~b~> (n3::n4::nil)) \b* (b3 ~b~> (n5::nil)) ) ->
+  triple (CopyFile f)
+    (\R[Hf,Hb])
+    (fun r => \exists f1 b4 b5 b6,( \[r= (val_floc f1)] \* 
+               (\R[(f1 ~f~> (b4::b5::b6::nil) \f* Hf ), 
+                   (b4 ~b~> (n1::n2::nil)) \b* (b5 ~b~> (n3::n4::nil))
+                   \b* (b6 ~b~> (n5::nil)) \b* Hb ]))).
+Proof.
+  intros. applys* triple_app_fun. simpl. subst.
+  applys triple_let. applys* triple_ReadFile. ext.
+  applys triple_conseq_frame triple_Create_File.
+  rewrite hstar_hempty_l'. applys himpl_refl. intros r.
+  ext_blk. intros f1. ext_blk. intros b4.
+  ext_blk. intros b5. ext_blk. intros b6.
+  rewrite hstar_assoc, hstar_sep, hbstar_assoc, hbstar_assoc.
+  intros h M. exists~ f1 b4 b5 b6.
 Qed.
