Language.v
@@ -4,7 +4,7 @@ This file describes the representation of modelling language.
 
 Author: Bowen Zhang.
 
-Date : 2022.01.06
+Date : 2023.02.21
 *)
 
 From SLF (* TLC *) Require Export LibCore.
@@ -12,67 +12,85 @@ From SLF (* Sep *) Require Export TLCbuffer Var Fmap.
 
 (* ###################### Syntax ###################### *)
 
-Definition loc : Type := nat.
 Definition bloc : Type := nat.
 Definition floc : Type := nat.
-
-Definition listint : Type := list int.
-Definition listbloc : Type := list bloc.
 
 Definition fnull : floc := 0%nat.
 Definition bnull : bloc := 0%nat.
 
 (*---------- the block primitive operations ----------*)
-Inductive bval : Type :=
-  | bval_create : bval
-  | bval_append : bval  
-  | bval_get : bval
-  | bval_delete : bval
-  | bval_bsize : bval
-  | bval_truncate : bval.
+Inductive bprim : Type :=
+  | bprim_create   : bprim   
+  | bprim_delete   : bprim   
+  | bprim_get      : bprim   
+  | bprim_size     : bprim  
+  | bprim_append   : bprim    
+  | bprim_trun     : bprim     
+  | bMR_mapper     : bprim.     (* WordCount mapper *)
 
 (*---------- the file primitive operations ----------*)
-Inductive fval : Type :=
-  | fval_create : fval
-  | fval_attach : fval
-  | fval_fsize : fval
-  | fval_get : fval
-  | fval_get_nth_blk : fval
-  | fval_set_nth_blk : fval
-  | fval_delete : fval
-  | fval_truncate : fval
-  (* some aux file operation *)
-  | fval_buffer: fval
-  | fval_buffer_list : fval
-  | fval_rev_blist : fval.
+Inductive fprim : Type :=
+  | fprim_create   : fprim 
+  | fprim_delete   : fprim     
+  | fprim_get      : fprim      
+  | fprim_size     : fprim     
+  | fprim_nthblk   : fprim    
+  | fprim_set      : fprim    
+  | fprim_attach   : fprim  
+  | fprim_trun     : fprim  
+  (*-- WordCount opertions --*)
+  | fMR_merge      : fprim
+  | fMR_group      : fprim
+  | fMR_reducer    : fprim.
 
-(*-------- some auxiliary primitive operations (not important) --------*)
-Inductive prim : Type :=
-  | val_eq : prim        (*a ?= b*)
-  | val_add : prim       (*a + b*)
-  | val_min : prim       (*a - b*)
-  | val_le : prim       (*a <= b*)
-  | val_list_rev : prim    (*reverse a list*)
-  | val_list_hd  : prim    (*extract list for a block*)
-  | val_list_len : prim   (*get the length of content*)
-  | val_list_tl  : prim    (*after extraction*)
-  | val_list_app : prim    (*append a list*)
-  | val_list_cut : prim.   (*truncate a list*)
+(*--------- arith operations -------------------*)
+Inductive aprim : Type :=
+  | val_eq  : aprim       (*a ?= b*)
+  | val_add : aprim       (*a + b*)
+  | val_min : aprim       (*a - b*)
+  | val_le  : aprim.      (*a <= b*)
+
+
+(*--------- WordCount values ---------*)
+(* wordcount kvpair (word, times) *)
+Definition wdpair : Type := int * int.
+
+Inductive WCval : Type :=
+  | WCval_listwdpair : list wdpair -> WCval
+  | WCval_Listwd : (list (list wdpair)) -> WCval.
+
+(*-------- some auxiliary list primitive operations (not important) --------*)
+Inductive lprim : Type :=
+  | val_list_rev     : lprim   (*reverse a list*)
+  | val_list_len     : lprim   (*get the length of content*)
+  | val_new_blist    : lprim   (*create a list of block locs*)
+  | val_blist_buffer : lprim   (*gather a list of block locs*)
+  | val_blist_rev    : lprim   (*reverse a list of block locs*)
+  | val_list_hd_bk   : lprim   (*extract list for a block*)
+  | val_list_tl_bk   : lprim   (*after extraction*)
+  | val_list_hd      : lprim   (*extract list for a block*)
+  | val_list_tl      : lprim   (*after extraction*)
+  | val_list_app     : lprim   (*append a list*)
+  | val_list_cut     : lprim   (*truncate a list*)
+  | val_reform       : lprim   (*trans list to save*)
+  | val_app_wdlist   : lprim.  (*append a word list*)
 
 (*---------- the val and the term ----------*)
 Inductive val : Type :=
-  | val_unit : val
-  | val_prim : prim -> val
-  | val_bool : bool -> val
-  | val_int : int -> val
-  | val_listint : list int -> val
+  | val_unit     : val
+  | val_bool     : bool -> val
+  | val_int      : int -> val
+  | val_listint  : list int -> val
   | val_listbloc : list bloc -> val
-  | val_floc : floc -> val
-  | val_bloc : bloc -> val
-  | val_bval : bval -> val
-  | val_fval : fval -> val
-  | val_fun : var -> trm -> val
-  | val_fix : var -> var -> trm -> val
+  | val_floc     : floc -> val
+  | val_bloc     : bloc -> val
+  | val_bprim    : bprim -> val
+  | val_fprim    : fprim -> val
+  | val_lprim    : lprim -> val
+  | val_aprim    : aprim -> val
+  | val_fun      : var -> trm -> val
+  | val_fix      : var -> var -> trm -> val
+  | val_WCval    : WCval -> val
 
 with trm : Type :=
   | trm_val : val -> trm
@@ -82,13 +100,12 @@ with trm : Type :=
   | trm_app : trm -> trm -> trm
   | trm_seq : trm -> trm -> trm
   | trm_let : var -> trm -> trm -> trm
-  | trm_if : trm -> trm -> trm -> trm
-  | trm_while : trm -> trm -> trm.
+  | trm_if  : trm -> trm -> trm -> trm.
 
 (* ##################### The Definition of CBS heap ##################### *)
 (*------- the entire corresponding state -------*)
-Definition stateb : Type := fmap bloc listint.
-Definition statef : Type := fmap floc listbloc.
+Definition stateb : Type := fmap bloc (list int).
+Definition statef : Type := fmap floc (list bloc).
 Definition state : Type := statef * stateb.
 
 (*------- the part of corresponding state -------*)
@@ -96,9 +113,9 @@ Definition heapb : Type := stateb.
 Definition heapf : Type := statef.
 Definition heap : Type := state.
 
-Notation "'hb_empty'" := (@Fmap.empty bloc listint)
+Notation "'hb_empty'" := (@Fmap.empty bloc (list int) )
   (at level 0).
-Notation "'hf_empty'" := (@Fmap.empty floc listbloc)
+Notation "'hf_empty'" := (@Fmap.empty floc (list bloc) )
   (at level 0).
 Notation "'h_empty'" := (hf_empty,hb_empty)
   (at level 0).
@@ -107,25 +124,28 @@ Notation "h1 \u h2" := (Fmap.union h1 h2)
 
 (*** Implicit Types and coercions (to improve the readability) ***)
 
-Implicit Types bp : bloc.
-Implicit Types fp : floc.
+Implicit Types b  : bloc.
+Implicit Types f  : floc.
 Implicit Types ln : list int.
-Implicit Types n : int.
-Implicit Types v : val.
-Implicit Types t : trm.
-Implicit Types b : bool.
+Implicit Types lb : list bloc.
+Implicit Types n w : int.
+Implicit Types v  : val.
+Implicit Types t  : trm.
+Implicit Types be : bool.
 Implicit Types hb : heapb.
 Implicit Types sb : stateb.
 Implicit Types hf : heapf.
 Implicit Types sf : statef.
 
-Coercion val_bool : bool >-> val.
-Coercion val_floc : floc >-> val.
-Coercion val_bloc : bloc >-> val.
-Coercion val_prim : prim >-> val.
-Coercion val_int : Z >-> val.
-Coercion val_bval : bval >-> val.
-Coercion val_fval : fval >-> val.
+Coercion val_bool  : bool >-> val.
+Coercion val_floc  : floc >-> val.
+Coercion val_bloc  : bloc >-> val.
+Coercion val_lprim : lprim >-> val.
+Coercion val_aprim : aprim >-> val.
+Coercion val_WCval : WCval >-> val.
+Coercion val_int   : Z >-> val.
+Coercion val_bprim : bprim >-> val.
+Coercion val_fprim : fprim >-> val.
 
 Coercion trm_val : val >-> trm.
 Coercion trm_var : var >-> trm.
@@ -145,17 +165,59 @@ Fixpoint subst (y:var) (w:val) (t:trm) : trm :=
   | trm_seq t1 t2 => trm_seq  (aux t1) (aux t2)
   | trm_let x t1 t2 => trm_let x (aux t1) (if_y_eq x t2 (aux t2))
   | trm_if t0 t1 t2 => trm_if (aux t0) (aux t1) (aux t2)
-  | trm_while t1 t2 => trm_while (aux t1) (aux t2)
   end.
 
 Definition trm_is_val (t:trm) : Prop :=
   match t with trm_val v => True | _ => False end.
 
-(**--------List Function--------**)
+(**--------some Coq functions to handel lists--------**)
 Definition droplast (n:nat) {A} (l:list A) : list A :=
   let l' := rev l in
   let l'' := drop n l' in
     rev l''.
+
+Definition init (w:int) : wdpair := (w,1).
+
+Definition app (l1 l2 : list wdpair) : list wdpair := List.app l1 l2.
+
+Definition lwdhd (lwd:list wdpair) : wdpair := (nth_default (0,0) 0 lwd).
+
+Definition eqword (p1 p2: wdpair) : bool := (fst p1) =? (fst p2).
+
+Definition neqword (p1 p2: wdpair) : bool := negb (eqword p1 p2).
+
+Definition neqlist (l1 l2:list wdpair) : bool := neqword (lwdhd l1) (lwdhd l2).
+
+Fixpoint classify (l1 l2:list wdpair) : list (list wdpair) :=
+  match l1,l2 with
+  | nil,_ | _, nil => nil
+  | x::l1',l2 => (List.filter (eqword x) l2) :: 
+    (classify l1' l2) 
+  end.
+
+Definition remove (lwd:list wdpair) (Lwd:list (list wdpair)) : list (list wdpair) := 
+ List.filter (neqlist lwd) Lwd.
+
+Fixpoint remove_duplicates (L:list (list wdpair)) : list (list wdpair):=
+  match L with
+  | nil => nil
+  | x::L' => x :: (remove x (remove_duplicates L'))
+  end.
+
+Definition addint (n1 n2:int) : int := n1+n2.
+
+Definition inithd (a:wdpair) : wdpair := ((fst a), 0).
+
+Definition addpair (a1 a2:wdpair) : wdpair := ((fst a1), (addint (snd a1) (snd a2) )).
+
+Definition accmulate (lwd:list wdpair) : wdpair :=
+  List.fold_right addpair (inithd (lwdhd lwd)) lwd.
+
+Fixpoint kv2int (l:list wdpair) : (list int) :=
+  match l with
+  | nil => nil
+  | (w,n) :: tl => w :: n :: (kv2int tl)
+end.
 
 (* ########################### The Evaluation Rules ########################### *)
 Open Scope liblist_scope.
@@ -169,10 +231,10 @@ Inductive eval : heap -> trm -> heap -> val -> Prop :=
       eval s (trm_val v) s v
   | eval_fun : forall s x t1,
       eval s (trm_fun x t1) s (val_fun x t1)
-  | eval_fix : forall s f x t1,
-      eval s (trm_fix f x t1) s (val_fix f x t1)
+  | eval_fix : forall s F x t1,
+      eval s (trm_fix F x t1) s (val_fix F x t1)
 
-  (*------   aux prim operation    ------*)
+  (*------   arith prim operation    ------*)
   | eval_add : forall s n1 n2,
       eval s (val_add n1 n2) s (n1 + n2)
   | eval_min : forall s n1 n2,
@@ -181,97 +243,97 @@ Inductive eval : heap -> trm -> heap -> val -> Prop :=
       eval s (val_le n1 n2) s (val_bool (isTrue (n1 <= n2)))
   | eval_eq : forall s n1 n2,
       eval s (val_eq n1 n2) s (val_bool (n1 =? n2))
-  | eval_list_rev : forall s l1,
-      eval s (val_list_rev (val_listint l1)) s (val_listint (rev l1))
-  
-  | eval_list_hd : forall s l1,
-      eval s (val_list_hd (val_listint l1)) s (val_listint (LibList.take 2%nat l1))
-  | eval_list_tl : forall s l1,
-      eval s (val_list_tl (val_listint l1)) s (val_listint (LibList.drop 2%nat l1))
-  | eval_list_len : forall s l1,
-      eval s (val_list_len (val_listint l1)) s (LibList.length l1)  
 
-  | eval_list_app : forall s l1 l2,
-      eval s (val_list_app (val_listint l1) (val_listint l2)) 
-           s (val_listint (l1 ++ l2))
+  (*------   aux prim operation    ------*)
+  | eval_list_rev : forall s ln1,
+      eval s (val_list_rev (val_listint ln1)) s (val_listint (rev ln1))
+  | eval_list_hd : forall s ln1,
+      eval s (val_list_hd (val_listint ln1)) s (val_listint (LibList.take 1%nat ln1))
+  | eval_list_tl : forall s ln1,
+      eval s (val_list_tl (val_listint ln1)) s (val_listint (LibList.drop 1%nat ln1))
+  | eval_list_hd_blk : forall s ln1,
+      eval s (val_list_hd_bk (val_listint ln1)) s (val_listint (LibList.take 2%nat ln1))
+  | eval_list_tl_blk : forall s ln1,
+      eval s (val_list_tl_bk (val_listint ln1)) s (val_listint (LibList.drop 2%nat ln1))
+  | eval_list_len : forall s ln1,
+      eval s (val_list_len (val_listint ln1)) s (LibList.length ln1)  
+  | eval_list_app : forall s ln1 ln2,
+      eval s (val_list_app (val_listint ln1) (val_listint ln2)) 
+           s (val_listint (ln1 ++ ln2))
+  | eval_blist_rev : forall sf sb bl,
+      eval (sf, sb) (val_blist_rev (val_listbloc bl)) (sf, sb) (val_listbloc (LibList.rev bl))
+  | eval_new_blist : forall sf sb b,
+      eval (sf, sb) (val_new_blist (val_bloc b)) (sf, sb) (val_listbloc (b::nil))
+  | eval_blist_buffer : forall sf sb b lb,
+      eval (sf, sb) (val_blist_buffer (val_bloc b) (val_listbloc lb)) (sf, sb) (val_listbloc (b::lb))
+
 
   (*--------- block prim operation ---------*)
-  | eval_bcreate_list : forall sf sb bp ll,
-      ~ Fmap.indom sb bp ->
-      eval (sf, sb) (bval_create (val_listint ll))
-        (sf, (Fmap.update sb bp ll)) (val_bloc bp)
+  | eval_bcreate : forall sf sb b ln,
+      ~ Fmap.indom sb b ->
+      eval (sf, sb) (bprim_create (val_listint ln)) (sf, (Fmap.update sb b ln)) b
 
-  | eval_bget : forall sf sb bp,
-      Fmap.indom sb bp ->
-      eval (sf, sb) (bval_get (val_bloc bp)) (sf, sb) (val_listint (Fmap.read sb bp))
+  | eval_bget : forall sf sb b,
+      Fmap.indom sb b ->
+      eval (sf, sb) (bprim_get (val_bloc b)) (sf, sb) (val_listint (Fmap.read sb b))
 
-  | eval_bdelete : forall sf sb bp,
-      Fmap.indom sb bp ->
-      eval (sf, sb) (bval_delete (val_bloc bp)) (sf, (Fmap.remove sb bp)) val_unit
+  | eval_bdelete : forall sf sb b,
+      Fmap.indom sb b ->
+      eval (sf, sb) (bprim_delete (val_bloc b)) (sf, (Fmap.remove sb b)) val_unit
 
-  | eval_bsize : forall sf sb bp,
-      Fmap.indom sb bp ->
-      eval (sf, sb) (bval_bsize (val_bloc bp))
-           (sf, sb) (val_int (List.length (Fmap.read sb bp)))
+  | eval_bsize : forall sf sb b,
+      Fmap.indom sb b ->
+      eval (sf, sb) (bprim_size (val_bloc b))
+           (sf, sb) (val_int (List.length (Fmap.read sb b)))
 
-  | eval_btruncate : forall sf sb bp n,
-      Fmap.indom sb bp ->
-      eval (sf, sb) (bval_truncate (val_bloc bp) n) 
-        (sf, (Fmap.update sb bp (droplast (Z.to_nat n) (Fmap.read sb bp) )))  val_unit
+  | eval_btruncate : forall sf sb b n,
+      Fmap.indom sb b ->
+      eval (sf, sb) (bprim_trun (val_bloc b) n) 
+        (sf, (Fmap.update sb b (droplast (Z.to_nat n) (Fmap.read sb b) )))  val_unit
 
-  | eval_bappend_list : forall sf sb bp ll,
-      Fmap.indom sb bp ->
-      eval (sf, sb) (bval_append (val_bloc bp) (val_listint ll)) 
-        (sf, (Fmap.update sb bp ((Fmap.read sb bp) ++ ll) ))  val_unit
+  | eval_bappend_list : forall sf sb b ln,
+      Fmap.indom sb b ->
+      eval (sf, sb) (bprim_append (val_bloc b) (val_listint ln)) 
+        (sf, (Fmap.update sb b ((Fmap.read sb b) ++ ln) ))  val_unit
 
  (*----------- file prim operation -----------*)
-  | eval_fcreate_list : forall sf sb fp bll,
-      ~ Fmap.indom sf fp ->
-      noduplicates bll ->
-      eval (sf, sb) (fval_create (val_listbloc bll))
-        ((Fmap.update sf fp bll), sb) (val_floc fp)
+  | eval_fcreate : forall sf sb f lb,
+      ~ Fmap.indom sf f ->
+      eval (sf, sb) (fprim_create (val_listbloc lb))
+        ((Fmap.update sf f lb), sb) (val_floc f)
 
-  | eval_fget : forall sf sb fp,
-      Fmap.indom sf fp ->
-      eval (sf, sb) (fval_get (val_floc fp)) (sf, sb) (val_listbloc (Fmap.read sf fp))
+  | eval_fget : forall sf sb f,
+      Fmap.indom sf f ->
+      eval (sf, sb) (fprim_get (val_floc f)) (sf, sb) (val_listbloc (Fmap.read sf f))
 
-  | eval_fsize : forall sf sb fp,
-      Fmap.indom sf fp ->
-      eval (sf, sb) (fval_fsize (val_floc fp))
-           (sf, sb) (val_int (List.length (Fmap.read sf fp)))
+  | eval_fsize : forall sf sb f,
+      Fmap.indom sf f ->
+      eval (sf, sb) (fprim_size (val_floc f))
+           (sf, sb) (val_int (List.length (Fmap.read sf f)))
 
-  | eval_fget_nth_blk : forall sf sb fp n,
-      Fmap.indom sf fp ->
-      eval (sf, sb) (fval_get_nth_blk (val_floc fp) n) (sf, sb)
-           (val_bloc (nth_default bnull (Z.to_nat n) (Fmap.read sf fp)))
+  | eval_fget_nth_blk : forall sf sb f n,
+      Fmap.indom sf f ->
+      eval (sf, sb) (fprim_nthblk (val_floc f) n) (sf, sb)
+           (val_bloc (nth_default bnull (Z.to_nat n) (Fmap.read sf f)))
 
-  | eval_fset_nth_blk : forall sf sb fp n bp,
-      Fmap.indom sf fp ->
-      eval (sf, sb) (fval_set_nth_blk (val_floc fp) n (val_bloc bp))
-           (Fmap.update sf fp (LibList.update (to_nat n) bp (Fmap.read sf fp)), sb) val_unit
+  | eval_fset_nth_blk : forall sf sb f n b,
+      Fmap.indom sf f ->
+      eval (sf, sb) (fprim_set (val_floc f) n (val_bloc b))
+           (Fmap.update sf f (LibList.update (to_nat n) b (Fmap.read sf f)), sb) val_unit
   
-  | eval_fattach: forall sf sb fp lb,
-      Fmap.indom sf fp ->
-      eval (sf, sb) (fval_attach (val_floc fp) (val_listbloc lb)) 
-       ((Fmap.update sf fp ( (Fmap.read sf fp) ++ lb )), sb) val_unit
+  | eval_fattach: forall sf sb f lb,
+      Fmap.indom sf f ->
+      eval (sf, sb) (fprim_attach (val_floc f) (val_listbloc lb)) 
+       ((Fmap.update sf f ( (Fmap.read sf f) ++ lb )), sb) val_unit
   
-  | eval_fdelete : forall sf sb fp,
-      Fmap.indom sf fp ->
-      eval (sf, sb) (fval_delete (val_floc fp)) ( (Fmap.remove sf fp), sb) val_unit
+  | eval_fdelete : forall sf sb f,
+      Fmap.indom sf f ->
+      eval (sf, sb) (fprim_delete (val_floc f)) ( (Fmap.remove sf f), sb) val_unit
 
-  | eval_frev_blist : forall sf sb bl,
-      eval (sf, sb) (fval_rev_blist (val_listbloc bl)) (sf, sb) (val_listbloc (LibList.rev bl))
-  
-  | eval_fbuffer : forall sf sb bp,
-      eval (sf, sb) (fval_buffer (val_bloc bp)) (sf, sb) (val_listbloc (bp::nil))
-
-  | eval_fbuffer_list : forall sf sb bp bl,
-      eval (sf, sb) (fval_buffer_list (val_bloc bp) (val_listbloc bl)) (sf, sb) (val_listbloc (bp::bl))
-
-  | eval_ftruncate : forall sf sb fp n,
-      Fmap.indom sf fp ->
-      eval (sf, sb) (fval_truncate (val_floc fp) n) 
-        ( (Fmap.update sf fp (droplast (Z.to_nat n) (Fmap.read sf fp) )), sb) val_unit
+  | eval_ftruncate : forall sf sb f n,
+      Fmap.indom sf f ->
+      eval (sf, sb) (fprim_trun (val_floc f) n) 
+        ( (Fmap.update sf f (droplast (Z.to_nat n) (Fmap.read sf f) )), sb) val_unit
 
   (*------------ trm rules ------------*)
    | eval_app_args : forall s1 s2 s3 s4 t1 t2 v1 v2 r,
@@ -284,9 +346,9 @@ Inductive eval : heap -> trm -> heap -> val -> Prop :=
       v1 = val_fun x t1 ->
       eval s1 (subst x v2 t1) s2 v ->
       eval s1 (trm_app v1 v2) s2 v
-   | eval_app_fix : forall s1 s2 v1 v2 f x t1 v,
-      v1 = val_fix f x t1 ->
-      eval s1 (subst x v2 (subst f v1 t1)) s2 v ->
+   | eval_app_fix : forall s1 s2 v1 v2 F x t1 v,
+      v1 = val_fix F x t1 ->
+      eval s1 (subst x v2 (subst F v1 t1)) s2 v ->
       eval s1 (trm_app v1 v2) s2 v
    | eval_seq : forall s1 s2 s3 t1 t2 v1 v,
       eval s1 t1 s2 v1 ->
@@ -296,12 +358,39 @@ Inductive eval : heap -> trm -> heap -> val -> Prop :=
       eval s1 t1 s2 v1 ->
       eval s2 (subst x v1 t2) s3 r ->
       eval s1 (trm_let x t1 t2) s3 r
-   | eval_if : forall s1 s2 b v t1 t2,
-      eval s1 (if b then t1 else t2) s2 v ->
-      eval s1 (trm_if (val_bool b) t1 t2) s2 v
-   | eval_while : forall s1 s2 t1 t2 v,
-      eval s1 (trm_if t1 (trm_seq t2 (trm_while t1 t2)) val_unit) s2 v ->
-      eval s1 (trm_while t1 t2) s2 v.
+   | eval_if : forall s1 s2 be v t1 t2,
+      eval s1 (if be then t1 else t2) s2 v ->
+      eval s1 (trm_if (val_bool be) t1 t2) s2 v
+
+  (*----- evaluation rules for MapReduce ------*)
+
+  (*-- mapper --*)
+  | eval_mapper : forall sf sb b,
+      Fmap.indom sb b ->
+      eval (sf, sb) (bMR_mapper b) (sf, sb) 
+        (WCval_listwdpair (List.map init (Fmap.read sb b)))
+
+  (*-- reducer --*)
+  | eval_merge : forall s Lwd,
+      eval s (fMR_merge (WCval_Listwd Lwd)) s (WCval_listwdpair (fold_right app nil Lwd))
+
+  | eval_group : forall s lwd,
+      eval s (fMR_group (WCval_listwdpair lwd)) s 
+        (WCval_Listwd (remove_duplicates (classify lwd lwd)))
+
+  | eval_wdreduce : forall s Lwd,
+      eval s (fMR_reducer (WCval_Listwd Lwd)) s (WCval_listwdpair (List.map accmulate Lwd))
+
+
+  (*-- aux rules for list operation in MapReduce --*)
+  | eval_app_wdlist : forall s lwd Lwd,
+      eval s (val_app_wdlist (WCval_listwdpair lwd) (WCval_Listwd Lwd)) 
+           s (WCval_Listwd (lwd :: Lwd))
+
+  | eval_reform : forall s lwd,
+      eval s (val_reform (WCval_listwdpair lwd)) s 
+        (val_listint (kv2int lwd)).
+
 
 (*  --------------- some relation about terms --------------- *)
 Definition eval_like (t1 t2:trm) : Prop :=
@@ -337,61 +426,61 @@ Qed.
 
 (*----------- block prim operations -----------*)
 
-Lemma eval_bcreate_sep : forall sf sb1 sb2 l bp,
-  sb2 = Fmap.single bp l ->
+Lemma eval_bcreate_sep : forall sf sb1 sb2 ln b,
+  sb2 = Fmap.single b ln ->
   Fmap.disjoint sb2 sb1 ->
-  eval (sf, sb1) (bval_create (val_listint l))
-       (sf, (Fmap.union sb2 sb1)) (val_bloc bp).
+  eval (sf, sb1) (bprim_create (val_listint ln))
+       (sf, (Fmap.union sb2 sb1)) (val_bloc b).
 Proof.
-  introv -> M. forwards Db: Fmap.indom_single bp l.
+  introv -> M. forwards Db: Fmap.indom_single b ln.
   rewrite <- Fmap.update_eq_union_single.
-  apply~ eval_bcreate_list.
+  apply~ eval_bcreate.
   { intros N. applys~ Fmap.disjoint_inv_not_indom_both M N. }
 Qed.
 
-Lemma eval_bget_sep : forall sf sb sb2 bp l,
-  sb = Fmap.union (Fmap.single bp l) sb2 ->
-  eval (sf, sb) (bval_get (val_bloc bp))
-       (sf, sb) (val_listint l).
+Lemma eval_bget_sep : forall sf sb sb2 b ln,
+  sb = Fmap.union (Fmap.single b ln) sb2 ->
+  eval (sf, sb) (bprim_get (val_bloc b))
+       (sf, sb) (val_listint ln).
 Proof.
-  introv ->. forwards Dv: Fmap.indom_single bp l.
+  introv ->. forwards Dv: Fmap.indom_single b ln.
   applys_eq eval_bget 1.
   { applys~ Fmap.indom_union_l. }
   { rewrite~ Fmap.read_union_l. rewrite~ Fmap.read_single. }
 Qed.
 
-Lemma eval_bsize_sep : forall sf sb sb2 bp l,
-  sb = Fmap.union (Fmap.single bp l) sb2 ->
-  eval (sf, sb) (bval_bsize (val_bloc bp))
-       (sf, sb) (List.length l).
+Lemma eval_bsize_sep : forall sf sb sb2 b ln,
+  sb = Fmap.union (Fmap.single b ln) sb2 ->
+  eval (sf, sb) (bprim_size (val_bloc b))
+       (sf, sb) (List.length ln).
 Proof.
-  introv ->. forwards Dv: Fmap.indom_single bp l.
+  introv ->. forwards Dv: Fmap.indom_single b ln.
   applys_eq eval_bsize 1.
   { applys~ Fmap.indom_union_l. }
   { rewrite~ Fmap.read_union_l. rewrite~ Fmap.read_single. }
 Qed.
 
-Lemma eval_bdelete_sep : forall sf sb1 sb2 bp l,
-  sb1 = Fmap.union (Fmap.single bp l) sb2 ->
-  Fmap.disjoint (Fmap.single bp l) sb2 ->
-  eval (sf, sb1) (bval_delete (val_bloc bp))
+Lemma eval_bdelete_sep : forall sf sb1 sb2 b ln,
+  sb1 = Fmap.union (Fmap.single b ln) sb2 ->
+  Fmap.disjoint (Fmap.single b ln) sb2 ->
+  eval (sf, sb1) (bprim_delete (val_bloc b))
        (sf, sb2) val_unit.
 Proof.
-  introv -> D. forwards Db: Fmap.indom_single bp l.
+  introv -> D. forwards Db: Fmap.indom_single b ln.
   applys_eq eval_bdelete 2.
   { applys~ Fmap.indom_union_l. }
   { rewrite~ Fmap.remove_union_single_l.
     intros D1. applys~ Fmap.disjoint_inv_not_indom_both D D1. }
 Qed.
 
-Lemma eval_btruncate_sep : forall sf sb1 sb2 sb bp l1 n,
-  sb1 = Fmap.union (Fmap.single bp l1) sb ->
-  sb2 = Fmap.union (Fmap.single bp (droplast (Z.to_nat n) l1)) sb ->
-  Fmap.disjoint (Fmap.single bp l1) sb ->
-  eval (sf, sb1) (bval_truncate (val_bloc bp) n)
+Lemma eval_btruncate_sep : forall sf sb1 sb2 sb b ln1 n,
+  sb1 = Fmap.union (Fmap.single b ln1) sb ->
+  sb2 = Fmap.union (Fmap.single b (droplast (Z.to_nat n) ln1)) sb ->
+  Fmap.disjoint (Fmap.single b ln1) sb ->
+  eval (sf, sb1) (bprim_trun (val_bloc b) n)
        (sf, sb2) val_unit.
 Proof.
-  introv -> -> D. forwards Db: Fmap.indom_single bp l1.
+  introv -> -> D. forwards Db: Fmap.indom_single b ln1.
   applys_eq eval_btruncate 2.
   { applys~ Fmap.indom_union_l. }
   { rewrite Fmap.read_union_l, Fmap.read_single; auto.
@@ -399,14 +488,14 @@ Proof.
     rewrite~ Fmap.update_single.  }
 Qed.
 
-Lemma eval_bappend_sep : forall sf sb1 sb2 sb bp l1 l2,
-  sb1 = Fmap.union (Fmap.single bp l1) sb ->
-  sb2 = Fmap.union (Fmap.single bp (l1++l2)) sb ->
-  Fmap.disjoint (Fmap.single bp l1) sb ->
-  eval (sf, sb1) (bval_append (val_bloc bp) (val_listint l2))
+Lemma eval_bappend_sep : forall sf sb1 sb2 sb bp ln1 ln2,
+  sb1 = Fmap.union (Fmap.single bp ln1) sb ->
+  sb2 = Fmap.union (Fmap.single bp (ln1++ln2)) sb ->
+  Fmap.disjoint (Fmap.single bp ln1) sb ->
+  eval (sf, sb1) (bprim_append (val_bloc bp) (val_listint ln2))
        (sf, sb2) val_unit.
 Proof.
-  introv -> -> D. forwards Db: Fmap.indom_single bp l1.
+  introv -> -> D. forwards Db: Fmap.indom_single bp ln1.
   applys_eq eval_bappend_list 2.
   { applys~ Fmap.indom_union_l. }
   { rewrite Fmap.read_union_l, Fmap.read_single; auto.
@@ -416,60 +505,59 @@ Qed.
 
 (*--------- file prim operations ---------*)
 
-Lemma eval_fcreate_sep : forall sf1 sb sf2 bll fp,
-  sf2 = Fmap.single fp bll ->
+Lemma eval_fcreate_sep : forall sf1 sb sf2 lb f,
+  sf2 = Fmap.single f lb ->
   Fmap.disjoint sf2 sf1 ->
-  noduplicates bll ->
-  eval (sf1, sb) (fval_create (val_listbloc bll))
-       ((Fmap.union sf2 sf1), sb) (val_floc fp).
+  eval (sf1, sb) (fprim_create (val_listbloc lb))
+       ((Fmap.union sf2 sf1), sb) (val_floc f).
 Proof.
-  introv -> D. forwards Db: Fmap.indom_single fp bll.
+  introv -> D. forwards Db: Fmap.indom_single f lb.
   rewrite <- Fmap.update_eq_union_single.
-  apply eval_fcreate_list.
+  apply eval_fcreate.
   { intros N. applys~ Fmap.disjoint_inv_not_indom_both D N. }
 Qed. 
 
-Lemma eval_fsize_sep : forall sf sb sf2 fp l,
-  sf = Fmap.union (Fmap.single fp l) sf2 ->
-  eval (sf, sb) (fval_fsize (val_floc fp))
-       (sf, sb) (List.length l).
+Lemma eval_fsize_sep : forall sf sb sf2 f lb,
+  sf = Fmap.union (Fmap.single f lb) sf2 ->
+  eval (sf, sb) (fprim_size (val_floc f))
+       (sf, sb) (List.length lb).
 Proof.
-  introv ->. forwards Dv: Fmap.indom_single fp l.
+  introv ->. forwards Dv: Fmap.indom_single f lb.
   applys_eq eval_fsize 1.
   { applys~ Fmap.indom_union_l. }
   { rewrite~ Fmap.read_union_l. rewrite~ Fmap.read_single. }
 Qed.
 
-Lemma eval_fget_sep : forall sf sb sf2 bll fp,
-  sf = Fmap.union (Fmap.single fp bll) sf2 ->
-  eval (sf, sb) (fval_get (val_floc fp))
-       (sf, sb) (val_listbloc bll).
+Lemma eval_fget_sep : forall sf sb sf2 lb f,
+  sf = Fmap.union (Fmap.single f lb) sf2 ->
+  eval (sf, sb) (fprim_get (val_floc f))
+       (sf, sb) (val_listbloc lb).
 Proof.
-  introv ->. forwards Df: Fmap.indom_single fp bll.
+  introv ->. forwards Df: Fmap.indom_single f lb.
   applys_eq eval_fget 1.
   { applys~ Fmap.indom_union_l. }
   { rewrite~ Fmap.read_union_l. rewrite~ Fmap.read_single. }
 Qed.
 
-Lemma eval_fget_nth_blk_sep : forall sf sb sf2 bll fp n,
-  sf = Fmap.union (Fmap.single fp bll) sf2 ->
-  eval (sf, sb) (fval_get_nth_blk (val_floc fp) n)
-       (sf, sb) (val_bloc (nth_default bnull (Z.to_nat n) bll)).
+Lemma eval_fget_nth_blk_sep : forall sf sb sf2 lb f n,
+  sf = Fmap.union (Fmap.single f lb) sf2 ->
+  eval (sf, sb) (fprim_nthblk (val_floc f) n)
+       (sf, sb) (val_bloc (nth_default bnull (Z.to_nat n) lb)).
 Proof.
-  introv ->. forwards Df: Fmap.indom_single fp bll.
+  introv ->. forwards Df: Fmap.indom_single f lb.
   applys_eq eval_fget_nth_blk 1.
   { applys~ Fmap.indom_union_l. }
   { rewrite~ Fmap.read_union_l. rewrite~ Fmap.read_single. }
 Qed.
 
-Lemma eval_fset_nth_blk_sep : forall sf sb sf1 sf2 bll fp n bp,
-  sf1 = Fmap.union (Fmap.single fp bll) sf ->
-  sf2 = Fmap.union (Fmap.single fp (LibList.update (to_nat n) bp bll)) sf ->
-  Fmap.disjoint (Fmap.single fp bll) sf ->
-  eval (sf1, sb) (fval_set_nth_blk (val_floc fp) n (val_bloc bp))
+Lemma eval_fset_nth_blk_sep : forall sf sb sf1 sf2 lb f n b,
+  sf1 = Fmap.union (Fmap.single f lb) sf ->
+  sf2 = Fmap.union (Fmap.single f (LibList.update (to_nat n) b lb)) sf ->
+  Fmap.disjoint (Fmap.single f lb) sf ->
+  eval (sf1, sb) (fprim_set (val_floc f) n (val_bloc b))
        (sf2, sb) (val_unit).
 Proof.
-  introv -> -> D. forwards Df: Fmap.indom_single fp bll.
+  introv -> -> D. forwards Df: Fmap.indom_single f lb.
   applys_eq eval_fset_nth_blk 2.
   { applys~ Fmap.indom_union_l. }
   { rewrite~ Fmap.update_union_l. fequals.
@@ -478,27 +566,27 @@ Proof.
     rewrite~ Fmap.read_single. }
 Qed.
 
-Lemma eval_fdelete_sep : forall sf1 sb sf2 bll fp,
-  sf1 = Fmap.union (Fmap.single fp bll) sf2 ->
-  Fmap.disjoint (Fmap.single fp bll) sf2 ->
-  eval (sf1, sb) (fval_delete (val_floc fp))
+Lemma eval_fdelete_sep : forall sf1 sb sf2 lb f,
+  sf1 = Fmap.union (Fmap.single f lb) sf2 ->
+  Fmap.disjoint (Fmap.single f lb) sf2 ->
+  eval (sf1, sb) (fprim_delete (val_floc f))
        (sf2, sb) val_unit.
 Proof.
-  introv -> D. forwards Df: Fmap.indom_single fp bll.
+  introv -> D. forwards Df: Fmap.indom_single f lb.
   applys_eq eval_fdelete 2.
   { applys~ Fmap.indom_union_l. }
   { rewrite~ Fmap.remove_union_single_l. intros D1.
     applys~  Fmap.disjoint_inv_not_indom_both D D1. }
 Qed.
 
-Lemma eval_fattach_sep : forall sf sf1 sf2 sb fp bl1 bl2,
-  sf1 = Fmap.union (Fmap.single fp bl1) sf ->
-  sf2 = Fmap.union (Fmap.single fp (bl1++bl2)) sf ->
-  Fmap.disjoint (Fmap.single fp bl1) sf ->
-  eval (sf1, sb) (fval_attach (val_floc fp) (val_listbloc bl2))
+Lemma eval_fattach_sep : forall sf sf1 sf2 sb f lb1 lb2,
+  sf1 = Fmap.union (Fmap.single f lb1) sf ->
+  sf2 = Fmap.union (Fmap.single f (lb1++lb2)) sf ->
+  Fmap.disjoint (Fmap.single f lb1) sf ->
+  eval (sf1, sb) (fprim_attach (val_floc f) (val_listbloc lb2))
        (sf2, sb) val_unit.
 Proof.
-  introv -> -> D. forwards Db: Fmap.indom_single fp bl1.
+  introv -> -> D. forwards Db: Fmap.indom_single f lb1.
   applys_eq eval_fattach 2.
   { applys~ Fmap.indom_union_l. }
   { rewrite Fmap.read_union_l, Fmap.read_single; auto.
@@ -506,14 +594,14 @@ Proof.
     rewrite~ Fmap.update_single. }
 Qed.
 
-Lemma eval_ftruncate_sep : forall sf sf1 sf2 sb fp bl n,
-  sf1 = Fmap.union (Fmap.single fp bl) sf ->
-  sf2 = Fmap.union (Fmap.single fp (droplast (Z.to_nat n) bl)) sf ->
-  Fmap.disjoint (Fmap.single fp bl) sf ->
-  eval (sf1, sb) (fval_truncate (val_floc fp) n)
+Lemma eval_ftruncate_sep : forall sf sf1 sf2 sb f lb n,
+  sf1 = Fmap.union (Fmap.single f lb) sf ->
+  sf2 = Fmap.union (Fmap.single f (droplast (Z.to_nat n) lb)) sf ->
+  Fmap.disjoint (Fmap.single f lb) sf ->
+  eval (sf1, sb) (fprim_trun (val_floc f) n)
        (sf2, sb) val_unit.
 Proof.
-  introv -> -> D. forwards Db: Fmap.indom_single fp bl.
+  introv -> -> D. forwards Db: Fmap.indom_single f lb.
   applys_eq eval_ftruncate 2.
   { applys~ Fmap.indom_union_l. }
   { rewrite Fmap.read_union_l, Fmap.read_single; auto.
@@ -521,7 +609,18 @@ Proof.
     rewrite~ Fmap.update_single. }
 Qed.
 
+(* ################### evaluation MR rule in SL style ############################## *)
 
+Lemma eval_wdmap_sep : forall sf sb sb2 b ln,
+  sb = Fmap.union (Fmap.single b ln) sb2 ->
+  eval (sf, sb) (bMR_mapper (val_bloc b))
+       (sf, sb) (WCval_listwdpair (List.map init ln)).
+Proof.
+  introv ->. forwards Dv: Fmap.indom_single b ln.
+  applys_eq eval_mapper 1.
+  { applys~ Fmap.indom_union_l. }
+  { rewrite~ Fmap.read_union_l. rewrite~ Fmap.read_single. }
+Qed.
 
 (*==============================================================*)
 (* ############ Notations of the language (to improve the readability) #################### *)
@@ -587,74 +686,62 @@ Notation "'Fun_' x1 x2 x3 ':=' t" :=
   (at level 69, x1, x2, x3 at level 0, format "'Fun_' x1 x2 x3 ':=' t") : trm_scope.
 
 (* ----------Notations of file prim---------------- *)
-Notation "'fcreate ll" :=
-  (fval_create ll)
+Notation "'fcreate lb" :=
+  (fprim_create lb)
   (at level 67) : trm_scope.
 
-Notation "'frev bl" :=
-  (fval_rev_blist bl)
+Notation "'fatt b lb" :=
+  (fprim_attach b lb)
+  (at level 67,b at level 0,format "''fatt' b lb").
+
+Notation "'set f n 'as b" :=
+  (fprim_set f n b)
+  (at level 67, f,b at level 0,format "''set' f n ''as' b") : trm_scope.
+
+Notation "'fsize f" :=
+  (fprim_size f)
   (at level 67) : trm_scope.
 
-Notation "'fbuffer p" :=
-  (fval_buffer p)
+Notation "'fdelete f" :=
+  (fprim_delete f)
   (at level 67) : trm_scope.
 
-Notation "'fatt bp l" :=
-  (fval_attach bp l)
-  (at level 67,bp at level 0,format "''fatt' bp l").
+Notation "'ftrun f n" :=
+  (fprim_trun f n)
+  (at level 67,f at level 0,format "''ftrun' f n") : trm_scope.
 
-Notation "'set_nth_blk fp n 'As bp" :=
-  (fval_set_nth_blk fp n bp)
-  (at level 67, fp,bp at level 0,format "''set_nth_blk' fp n ''As' bp") : trm_scope.
-
-Notation "'fsize p" :=
-  (fval_fsize p)
-  (at level 67) : trm_scope.
-
-Notation "'fdelete fp" :=
-  (fval_delete fp)
-  (at level 67) : trm_scope.
-
-Notation "'ftrun fp n" :=
-  (fval_truncate fp n)
-  (at level 67,fp at level 0,format "''ftrun' fp n") : trm_scope.
-
-Notation "'nth_blk fp n" :=
-  (fval_get_nth_blk fp n)
-  (at level 67, fp at level 0,format "''nth_blk' fp n") : trm_scope.
-
-Notation "bp 'b+ bl" :=
-  (fval_buffer_list bp bl)
-  (at level 67) : trm_scope.
+Notation "'nthblk f n" :=
+  (fprim_nthblk f n)
+  (at level 67, f at level 0,format "''nthblk' f n") : trm_scope.
 
 (* ----------Notations of block prim---------------- *)
-Notation "'bcreate ll" :=
-  (bval_create ll)
+Notation "'bcreate ln" :=
+  (bprim_create ln)
   (at level 67) : trm_scope.
 
-Notation "'bapp bp l" :=
-  (bval_append bp l)
-  (at level 67,bp at level 0,format "''bapp' bp l") : trm_scope.
+Notation "'bapp b ln" :=
+  (bprim_append b ln)
+  (at level 67,b at level 0,format "''bapp' b ln") : trm_scope.
 
-Notation "'bsize p" :=
-  (bval_bsize p)
+Notation "'bsize f" :=
+  (bprim_size f)
   (at level 67) : trm_scope.
 
-Notation "'bget bp" :=
-  (bval_get bp)
+Notation "'bget b" :=
+  (bprim_get b)
   (at level 67) : trm_scope.
 
-Notation "'bsize bp" :=
-  (bval_bsize bp)
+Notation "'bsize b" :=
+  (bprim_size b)
   (at level 67) : trm_scope.
 
-Notation "'bdelete bp" :=
-  (bval_delete bp)
+Notation "'bdelete b" :=
+  (bprim_delete b)
   (at level 67) : trm_scope.
 
-Notation "'btrun bp n" :=
-  (bval_truncate bp n)
-  (at level 67, bp at level 0,format "''btrun' bp n") : trm_scope.
+Notation "'btrun b n" :=
+  (bprim_trun b n)
+  (at level 67, b at level 0,format "''btrun' b n") : trm_scope.
 
 (* ----------Notations of aux prim---------------- *)
 Notation "n1 '= n2" :=
@@ -673,26 +760,75 @@ Notation "n1 '<= n2" :=
   (val_le n1 n2)
   (at level 67) : trm_scope.
 
-Notation "l1 '++ l2" :=
-  (val_list_app l1 l2)
+Notation "ln1 '++ ln2" :=
+  (val_list_app ln1 ln2)
   (at level 67) : trm_scope.
 
-Notation "'rev l1" :=
-  (val_list_rev l1)
+Notation "'rev ln1" :=
+  (val_list_rev ln1)
   (at level 67) : trm_scope.
 
-Notation "'hd l1" :=
-  (val_list_hd l1)
+Notation "'hd ln1" :=
+  (val_list_hd ln1)
   (at level 67) : trm_scope.
 
-Notation "'tl l1" :=
-  (val_list_tl l1)
+Notation "'tl ln1" :=
+  (val_list_tl ln1)
   (at level 67) : trm_scope.
 
-Notation "'len l1" :=
-  (val_list_len l1)
+Notation "'hdblk ln1" :=
+  (val_list_hd_bk ln1)
+  (at level 67) : trm_scope.
+
+Notation "'tlblk ln1" :=
+  (val_list_tl_bk ln1)
+  (at level 67) : trm_scope.
+
+Notation "'len ln1" :=
+  (val_list_len ln1)
+  (at level 67) : trm_scope.
+
+Notation "'frev lb" :=
+  (val_blist_rev lb)
+  (at level 67) : trm_scope.
+
+Notation "'buffer b" :=
+  (val_new_blist b)
+  (at level 67) : trm_scope.
+
+Notation "b 'b+ lb" :=
+  (val_blist_buffer b lb)
   (at level 67) : trm_scope.
 
 Notation "'()" := val_unit : trm_scope.
+
+(* ====== Notation for mapreduce ====== *)
+
+(* -- mapper -- *)
+Notation "'mapper b" :=
+  (bMR_mapper b)
+  (at level 67) : trm_scope.
+
+(* -- reducer -- *)
+Notation "'merge Lwd" :=
+  (fMR_merge Lwd)
+  (at level 67) : trm_scope.
+
+Notation "'group lwd" :=
+  (fMR_group lwd)
+  (at level 67) : trm_scope.
+
+Notation "'reducer Lwd" :=
+  (fMR_reducer Lwd)
+  (at level 67) : trm_scope.
+
+(*-- some aux list operations --*)
+Notation "l 'w:: L" :=
+  (val_app_wdlist l L)
+  (at level 67, format " l ''w::' L") : trm_scope.
+
+Notation "'reform lwd" :=
+  (val_reform lwd)
+  (at level 67) : trm_scope.
 
 End NotationForTrm.
