ExMapReduce.v
@@ -1,0 +1,504 @@
+(* ########################### MapReduce ########################### *)
+(**
+
+== Representation and verification of WordCount ==
+
+WordCount is a standard MapReduce application.
+It counts each word's frequency in a CBS file.
+
+This file shows how we represent the actual application, 
+and how we specify and verify the behavior of programs.
+
+Advice: readers need to read Language.v first.
+
+Author: Bowen Zhang.
+
+Date : 2022.11.1
+*)
+
+From SLF (* TLC *) Require Export LibCore TLCbuffer.
+From SLF (* Sep *) Require Export TripleAndRules ExBasic.
+(*------------------------------------------------------------------------*)
+
+Export NotationForTrm.
+Export NotationForVariables.
+
+Open Scope val_scope.
+Open Scope trm_scope.
+Open Scope Z_scope.
+
+(* ########################### WordCount ########################### *)
+
+(*  
+~~~~~~~~~~~~~~~~~~~~~~~~~~~~~~~~~~~
+Suppose a HDFS state before WordCount:
+
+--f
+  | bk1 [n1;n2]
+  | bk2 [n3;n1]
+  | bk3 [n2]
+
+~~~~~~~~~~~~~~~~~~~~~~~~~~~~~~~~~~~
+The state after WordCount:
+
+--f
+  | bk1 [n1;n2]
+  | bk2 [n3;n1]
+  | bk3 [n2]
+
+--f2
+  | bk4 [n1;2]
+  | bk5 [n2;2]
+  | bk6 [n3;1]
+*)
+
+(* 
+------- Representation and Specification ----------
+
+Definition WordCount := 
+  Fun 'f :=
+    Let 'L1 := Mapper 'f 0 in
+    Let 'L2 := Shuffle 'L1 in
+    Let 'l := Reducer 'L2 in
+    Create_File 'l.
+
+
+Lemma triple_WordCount: forall Hf Hb (f:floc) (n1 n2 n3 :int) (p1 p2 p3:bloc),
+  diff_each_3 n1 n2 n3 ->
+  Hf = ( f ~f~> (p1::p2::p3::nil) ) ->
+  Hb = ( (p1 ~b~> (n1::n2::nil)) \b* (p2 ~b~> (n3::n1::nil)) \b* (p3 ~b~> (n2::nil)) ) ->
+  triple (WordCount f)
+    (\R[Hf,Hb])
+    (fun r => \exists f1 b4 b5 b6,( \[r= (val_floc f1)] \* 
+        (\R[(f1 ~f~> (b4::b5::b6::nil) \f* Hf),
+        Hb \b* (b4 ~b~> (n1::2::nil)) \b* (b5 ~b~> (n2::2::nil))
+        \b* (b6 ~b~> (n3::1::nil))] ))).
+
+*)
+
+
+(*------------------------------------------------------------------------*)
+
+(*------------------------------------------------------------------------*)
+
+(* ================================================================= *)
+(** Some ltac to simplify the verification *)
+
+(*--- to extract the existential quantifier ---*)
+Ltac extexists :=
+  intros; simpl; 
+  try apply triple_hfexists;
+  try apply triple_hfexists';
+  try apply triple_hbexists;
+  try apply triple_hbexists';
+  try apply triple_hexists.
+
+(*--- to extract the pure fact ---*)
+Ltac extpure :=
+  intros; simpl; 
+  try apply triple_hfpure;
+  try apply triple_hbpure; 
+  try apply triple_hpure;
+  simpls;
+  intros ->.
+
+(* - combine the extraction - *)
+Ltac ext :=
+  try extpure; try extexists.
+
+(*--------- Some scripts for CBS-heap entailments --------------*)
+Ltac inner_femp :=
+ try intros r;
+ try rewrite hstar_sep;
+ try rewrite hfstar_hempty_l;
+ try rewrite hfstar_hempty_r;
+ apply himpl_refl.
+
+Ltac inner_bemp :=
+ try intros r;
+ try rewrite hstar_sep;
+ try rewrite hbstar_hempty_l;
+ try rewrite hbstar_hempty_r;
+ apply himpl_refl.
+
+Ltac outer_emp :=
+ try intros r;
+ try rewrite hstar_hempty_l';
+ try rewrite hstar_hempty_r';
+ apply himpl_refl.
+
+Ltac rew_read:=
+  intros v;
+  rewrite hstar_assoc,hstar_sep,hfstar_hempty_l;
+  apply himpl_refl;
+  ext.
+
+(*--------- Some scripts for recursive programs --------------*)
+Lemma nth_listbloc_1 : forall p1 p2 p3,
+(nth_default bnull (to_nat 1) (p1 :: p2 :: p3 :: nil)) = p2.
+Proof.
+  intros. rewrite to_nat_1,nth_default_succ,nth_default_zero. auto.
+Qed.
+
+Lemma nth_listbloc_1' : forall p1 p2,
+(nth_default bnull (to_nat 1) (p1 :: p2 :: nil)) = p2.
+Proof.
+  intros. rewrite to_nat_1,nth_default_succ,nth_default_zero. auto.
+Qed.
+
+Lemma nth_listbloc_2 : forall p1 p2 p3,
+(nth_default bnull (to_nat (1 + 1)) (p1 :: p2 :: p3 :: nil)) = p3.
+Proof.
+  intros. rewrite to_nat_plus; try math.
+  rewrite to_nat_1. do 2 rewrite nth_default_succ. rewrite~ nth_default_zero.
+Qed.
+
+(*----- expand the recursive program  -------*)
+Ltac exp_fix :=
+  intros; subst; applys* triple_app_fix2; simpl;
+  applys triple_let triple_fsize; ext;
+  applys triple_let triple_eq; ext;
+  applys triple_if; case_if*.
+
+(*----- verify rec body until to the target block -------*)
+Ltac fix_body := 
+  applys triple_let triple_fget_nth_blk; ext;
+  applys triple_let triple_add; ext;
+  try rewrite nth_default_zero;
+  try rewrite nth_listbloc_1;
+  try rewrite nth_listbloc_1';
+  try rewrite nth_listbloc_2.
+
+(* ------ for read file example --------- *)
+Ltac fix_read :=
+  exp_fix; fix_body;
+  applys triple_let;
+  try applys triple_conseq_frame triple_bget.
+
+(* ------ for map file example --------- *)
+Ltac fix_map :=
+  exp_fix; fix_body;
+  applys triple_let;
+  try applys triple_conseq_frame triple_wdmap.
+
+
+(* ------ for remove file example --------- *)
+Ltac fix_rem :=
+  exp_fix; fix_body;
+  applys triple_seq;
+  try applys triple_conseq_frame triple_bdelete.
+
+(* ################################## *)
+Lemma eqword_refl : forall n1,
+  eqword (n1,1) (n1,1) = true.
+Proof. intros. unfold eqword. simpl. apply~ Z.eqb_eq. Qed.
+
+Lemma neqword_refl : forall n1,
+  neqword (n1,1) (n1,1) = false.
+Proof. intros. unfold neqword. rewrite~ eqword_refl. Qed.
+
+Lemma eqword_diff : forall n1 n2,
+  n1 =? n2 = false ->
+  eqword (n1,1) (n2,1) = false.
+Proof. intros. unfold eqword. simpls~. Qed.
+
+Lemma eqb_comm : forall n1 n2,
+  (n1 =? n2) = (n2 =? n1).
+Proof.
+  intros. destruct (n1 =? n2) eqn:H.
+  apply Z.eqb_eq in H. rewrite H.
+  symmetry. apply~ Z.eqb_eq.
+  symmetry. apply Bool.not_true_is_false.
+  intro N.  apply Z.eqb_eq in N.
+  rewrite N in H. lets : Z.eqb_eq n1 n1.
+  assert (H1: n1 = n1). auto.
+  apply H0 in H1. rewrite H in H1. discriminate.
+Qed.
+
+Lemma eqword_diff_2 : forall n1 n2,
+  n1 =? n2 = false ->
+  eqword (n2,1) (n1,1) = false.
+Proof. intros. unfold eqword. simpls. rewrite~ eqb_comm. Qed.
+
+Lemma neqword_diff_2 : forall n1 n2,
+  n1 =? n2 = false ->
+  neqword (n2,1) (n1,1) = true.
+Proof. intros. unfold neqword. rewrite~ eqword_diff_2. Qed.
+
+Lemma neqword_diff : forall n1 n2,
+  n1 =? n2 = false ->
+  neqword (n1,1) (n2,1) = true.
+Proof. intros. unfold neqword. rewrite~ eqword_diff. Qed.
+
+Hint Resolve eqword_refl eqword_diff_2 eqb_comm neqword_diff_2 neqword_diff neqword_refl.
+
+Definition diff_each_3 (n1 n2 n3:int) : Prop :=
+  n1 =? n2 = false /\ n1 =? n3 = false /\ n2 =? n3 = false.
+
+Lemma diff_3_bool : forall n1 n2 n3,
+   diff_each_3 n1 n2 n3 ->
+   eqword (n1,1) (n1,1) = true
+/\ eqword (n2,1) (n2,1) = true
+/\ eqword (n3,1) (n3,1) = true
+/\ eqword (n1,1) (n2,1) = false
+/\ eqword (n1,1) (n3,1) = false
+/\ eqword (n2,1) (n3,1) = false
+/\ eqword (n2,1) (n1,1) = false
+/\ eqword (n3,1) (n1,1) = false
+/\ eqword (n3,1) (n2,1) = false.
+Proof. introv. intros (H1&H2&H3). splits*. Qed.
+
+Lemma classify_result: forall n1 n2 n3 lwd,
+diff_each_3 n1 n2 n3 ->
+lwd = ((n1, 1) :: (n2, 1) :: (n3, 1) :: (n1, 1) :: (n2, 1) :: nil) ->
+(classify lwd lwd) = 
+( ((n1,1)::(n1,1)::nil) :: ((n2,1)::(n2,1)::nil) :: ((n3,1)::nil) ::
+  ((n1,1)::(n1,1)::nil) :: ((n2,1)::(n2,1)::nil) :: nil ) .
+Proof.
+  intros. apply diff_3_bool in H
+  as (H1&H2&H3&H4&H5&H6&H7&H8&H9). subst.
+  unfold classify. repeat case_if.
+  simpl. repeat case_if. simpl. repeat case_if. simpls~.
+Qed.
+
+Lemma diff_3_list_bool : forall n1 n2 n3,
+   diff_each_3 n1 n2 n3 ->
+   neqlist ((n2, 1) :: (n2, 1) :: nil) ((n3, 1) :: nil) = true
+/\ neqlist ((n3, 1) :: nil) ((n1, 1) :: (n1, 1) :: nil) = true
+/\ neqlist ((n1, 1) :: (n1, 1) :: nil) ((n3, 1) :: nil) = true
+/\ neqlist ((n2, 1) :: (n2, 1) :: nil) ((n1, 1) :: (n1, 1) :: nil) = true
+/\ neqlist ((n3, 1) :: nil) ((n2, 1) :: (n2, 1) :: nil) = true
+/\ neqlist ((n1, 1) :: (n1, 1) :: nil) ((n1, 1) :: (n1, 1) :: nil) = false
+/\ neqlist ((n2, 1) :: (n2, 1) :: nil) ((n2, 1) :: (n2, 1) :: nil) = false
+/\ neqlist ((n1, 1) :: (n1, 1) :: nil) ((n2, 1) :: (n2, 1) :: nil) = true.
+Proof.
+  introv. intros (H1&H2&H3). unfold neqlist, lwdhd.
+  repeat rewrite nth_default_zero. splits*.
+Qed.
+
+Lemma shuffle_result: forall n1 n2 n3 lwd,
+diff_each_3 n1 n2 n3 ->
+lwd = ((n1, 1) :: (n2, 1) :: (n3, 1) :: (n1, 1) :: (n2, 1) :: nil) ->
+(remove_duplicates (classify lwd lwd)) = 
+( ((n1,1)::(n1,1)::nil) :: ((n2,1)::(n2,1)::nil) :: ((n3,1)::nil) ::nil ) .
+Proof.
+  intros. forwards T : classify_result H H0. rewrite T.
+  forwards (H1&H2&H3&H4&H5&H6&H7&H8) : diff_3_list_bool H.
+  unfold remove_duplicates. simpl. repeat case_if.
+  simpl. repeat case_if. simpl. repeat case_if. simpls~.
+Qed.
+
+
+
+(*============= Mapper ================*)
+Definition Mapper := 
+  Fix 'F 'f 'i :=
+    Let 'n := 'fsize 'f in
+    Let 'be := ('i '= 'n) in
+    If_ 'be
+    Then (WCval_Listwd nil)
+    Else
+      Let 'bk := 'nthblk 'f 'i in
+      Let 'i1 := 'i '+ 1 in
+      Let 'ln := 'mapper 'bk in
+      Let 'ln1 := 'F 'f 'i1 in
+      'ln 'w:: 'ln1.
+
+(* specification of mapper *)
+Lemma triple_Mapper: forall Hf Hb (f:floc) (n1 n2 n3:int) (p1 p2 p3:bloc) (L:(list (list wdpair))),
+  diff_each_3 n1 n2 n3 ->
+  Hf = ( f ~f~> (p1::p2::p3::nil) ) ->
+  Hb = ( (p1 ~b~> (n1::n2::nil)) \b* (p2 ~b~> (n3::n1::nil)) \b* (p3 ~b~> (n2::nil)) ) ->
+  L = ( ((n1,1)::(n2,1)::nil) :: ((n3,1)::(n1,1)::nil) :: ((n2,1)::nil) :: nil ) ->
+  triple (Mapper f 0)
+    (\R[Hf,Hb])
+    (fun r => \[r= WCval_Listwd L] \* \R[Hf,Hb]).
+Proof.
+  fix_map.
+  rewrite hstar_sep, hfstar_hempty_l. apply himpl_refl.
+  rew_read. ext.
+
+  applys triple_let.
+  fix_map.
+  rewrite hstar_sep, hfstar_hempty_l,hbstar_comm,hbstar_assoc. apply himpl_refl.
+  rew_read. ext.
+
+  applys triple_let.
+  fix_map.
+  rewrite hstar_sep, hfstar_hempty_l,hbstar_comm,hbstar_assoc. apply himpl_refl.
+  rew_read. ext.
+
+  applys triple_let.
+  exp_fix.
+  applys triple_val'. ext.
+  applys triple_app_wdlist. ext.
+  applys triple_app_wdlist. ext.
+  applys triple_conseq triple_app_wdlist.
+  apply himpl_refl.
+  intros r. rew_list. 
+  rewrite hbstar_comm,hbstar_assoc. apply himpl_refl.
+Qed.
+
+(*============= Shuffle ================*)
+Definition Shuffle :=
+ Fun 'L :=
+    Let 'l := 'merge 'L in
+      'group 'l.
+
+Lemma triple_Shuffle: forall Hf Hb (n1 n2 n3 : int) (L1 L2: (list (list wdpair))),
+  diff_each_3 n1 n2 n3 ->
+  L1 = ( ((n1,1)::(n2,1)::nil) :: ((n3,1)::(n1,1)::nil) :: ((n2,1)::nil) :: nil ) ->
+  L2 = ( ((n1,1)::(n1,1)::nil) :: ((n2,1)::(n2,1)::nil) :: ((n3,1)::nil) ::nil ) ->
+  triple (Shuffle (WCval_Listwd L1))
+    (\R[Hf,Hb])
+    (fun r => \[r= WCval_Listwd L2] \* \R[Hf,Hb]).
+Proof.
+  intros. subst.
+  applys* triple_app_fun. simpl.
+  applys triple_let.
+  applys triple_conseq_frame triple_wdmerge.
+  rewrite hstar_hempty_r'. applys himpl_refl.
+  intros r. rewrite hstar_hempty_r'. simpl. applys himpl_refl.
+  ext.
+  applys triple_conseq_frame triple_wdgroup.
+  rewrite hstar_hempty_r'. applys himpl_refl.
+  intros r. rewrite hstar_hempty_r'.
+  eapply shuffle_result in H. rewrite <- H.
+  applys* himpl_refl. auto.
+Qed.
+
+(*============= Reducer ================*)
+Definition Reducer :=
+  Fun 'L :=  'reducer 'L.
+
+Lemma triple_Reducer: forall Hf Hb (n1 n2 n3 : int) (lwd:list wdpair) (L : (list (list wdpair))),
+  diff_each_3 n1 n2 n3 ->
+  L = ( ((n1,1)::(n1,1)::nil) :: ((n2,1)::(n2,1)::nil) :: ((n3,1)::nil) ::nil ) ->
+  lwd = ((n1,2)::(n2,2)::(n3,1)::nil ) ->
+  triple (Reducer (WCval_Listwd L))
+    (\R[Hf,Hb])
+    (fun r => \[r= WCval_listwdpair lwd] \* \R[Hf,Hb]).
+Proof.
+  intros. subst.
+  applys* triple_app_fun. simpl.
+  applys triple_conseq_frame triple_wdreduce.
+  rewrite hstar_hempty_r'. applys himpl_refl.
+  intros r. rewrite hstar_hempty_r'.
+  applys himpl_refl.
+Qed.
+
+
+(*============= Create files ================*)
+
+Lemma triple_CreateBlks' : forall Hf (n1 n2 n3 n4 n5 n6:int),
+  triple (CreateBlks (val_listint (n1::n2::n3::n4::n5::n6::nil)) (val_listbloc nil))
+    (\R[Hf, \b[] ])
+     (fun r => \exists b1 b2 b3,( \[r=(val_listbloc (b3::b2::b1::nil))] \* 
+               (\R[Hf, (b1 ~b~> (n1::n2::nil)) \b* (b2 ~b~> (n3::n4::nil) \b* (b3 ~b~> (n5::n6::nil)))]))).
+Proof.
+  cre_exp_fix. destruct C. auto.
+  applys triple_let triple_list_hd_bk. ext.
+  applys triple_let triple_list_tl_bk. ext.
+  applys triple_let.
+  applys triple_conseq_frame triple_bcreate.
+  cre_pre. intros r. apply himpl_refl.
+  cre_ext. intros b1.
+  rewrite hstar_hempty_r. ext.
+  applys triple_let triple_blist_buffer. ext.
+
+  exp_fix_create.
+  applys triple_conseq_frame triple_bcreate.
+  cre_pre. intros r. apply himpl_refl.
+  cre_ext. intros b2.
+  rewrite hstar_assoc, hstar_sep, hfstar_hempty_r. ext.
+  applys triple_let triple_blist_buffer. ext.
+
+  cre_exp_fix. applys triple_let.
+  applys triple_conseq_frame triple_bcreate.
+  rewrite hstar_sep, hfstar_hempty_r, hbstar_hempty_l. apply himpl_refl.
+  intros* r. apply himpl_refl. cre_ext. intros b3.
+  rewrite hstar_assoc, hstar_sep, hfstar_hempty_r. ext.
+  applys triple_conseq_frame triple_blist_buffer.
+  rewrite hstar_hempty_l'. apply himpl_refl.
+  intros r. rewrite hstar_hempty_r, hbstar_comm3.
+  intros h H. apply hstar_hpure_iff in H as (H1&H2).
+  exists b1 b2 b3.
+  applys hstar_hpure_iff. splits~.
+  destruct C1. rew_list. discriminate.
+Qed.
+
+Lemma triple_CreateFile' : forall (n1 n2 n3 n4 n5 n6:int),
+  triple (Create_File (val_listint (n1::n2::n3::n4::n5::n6::nil)) )
+    (\R[\f[], \b[] ])
+     (fun r => \exists f b1 b2 b3,( \[r= (val_floc f)] \* 
+               (\R[(f ~f~> (b1::b2::b3::nil)), (b1 ~b~> (n1::n2::nil)) \b* (b2 ~b~> (n3::n4::nil) \b* (b3 ~b~> (n5::n6::nil)))]))).
+Proof.
+  intros. applys* triple_app_fun.
+  applys triple_let triple_CreateBlks'.
+  intros v. ext. intros b1. ext. intros b2. ext. intros b3. ext.
+  applys triple_let.
+  applys triple_conseq_frame triple_blist_rev.
+  rewrite hstar_hempty_l'. apply himpl_refl.
+  intros r. rewrite hstar_assoc, hstar_hempty_l. apply himpl_refl.
+  ext.
+  applys triple_conseq_frame triple_fcreate.
+  rewrite hstar_hempty_r'. apply himpl_refl.
+  intros v. rewrite hstar_hempty_r'.
+  apply himpl_hexists_l. intros f.
+  intros h M. exists~ f b1 b2 b3.
+Qed.
+
+Definition SaveResult : val :=
+  Fun 'l:=
+    Let 'ln1 := 'reform 'l in
+      Create_File 'ln1.
+
+Lemma triple_SaveResult : forall (w1 w2 w3 n1 n2 n3:int),
+  triple (SaveResult (WCval_listwdpair ((w1,n1)::(w2,n2)::(w3,n3)::nil)) )
+    (\R[\f[], \b[] ])
+     (fun r => \exists f b1 b2 b3,( \[r= (val_floc f)] \* 
+               (\R[(f ~f~> (b1::b2::b3::nil)), (b1 ~b~> (w1::n1::nil)) \b* (b2 ~b~> (w2::n2::nil) \b* (b3 ~b~> (w3::n3::nil)))]))).
+Proof.
+  intros. applys* triple_app_fun. simpl.
+  applys triple_let triple_MRlist_reform.
+  ext. apply triple_CreateFile'.
+Qed.
+
+
+
+(* $$$$$$$$$$$$$==================$$$$$$$$$$$$$$$$$$$$$ *)
+
+
+Definition WordCount := 
+  Fun 'f :=
+    Let 'L := Mapper 'f 0 in
+    Let 'L1 := Shuffle 'L in
+    Let 'lwd := Reducer 'L1 in
+    SaveResult 'lwd.
+
+Lemma triple_WordCount: forall Hf Hb (f:floc) (n1 n2 n3 :int) (p1 p2 p3:bloc),
+  diff_each_3 n1 n2 n3 ->
+  Hf = ( f ~f~> (p1::p2::p3::nil) ) ->
+  Hb = ( (p1 ~b~> (n1::n2::nil)) \b* (p2 ~b~> (n3::n1::nil)) \b* (p3 ~b~> (n2::nil)) ) ->
+  triple (WordCount f)
+    (\R[Hf,Hb])
+    (fun r => \exists f1 b4 b5 b6,( \[r= (val_floc f1)] \* 
+        (\R[(f1 ~f~> (b4::b5::b6::nil) \f* Hf),
+            (b4 ~b~> (n1::2::nil)) \b* (b5 ~b~> (n2::2::nil))
+        \b* (b6 ~b~> (n3::1::nil)) \b* Hb ] ))).
+Proof.
+  intros. subst.
+  applys* triple_app_fun. simpl.
+  applys triple_let.
+  applys* triple_Mapper.
+  simpl. intros r. ext.
+  applys triple_let. applys* triple_Shuffle H. ext.
+  applys triple_let. applys* triple_Reducer. ext.
+  applys triple_conseq_frame triple_SaveResult.
+  rewrite hstar_hempty_l'. apply himpl_refl. intros r.
+  ext_blk. intros f1. ext_blk. intros b4.
+  ext_blk. intros b5. ext_blk. intros b6.
+  rewrite hstar_assoc, hstar_sep, hbstar_assoc, hbstar_assoc.
+  intros h M. exists~ f1 b4 b5 b6.
+Qed.
+ 
