Hoare.v
@@ -1,0 +1,469 @@
+(**
+
+This file mainly describes the Hoare triple and the related rules.
+It helps us to construct our formal system.
+
+  1. the definitions of Hoare triple in CBS
+  2. the statement and prove of the reasoning rules for Hoare triples.
+
+Author: Bowen Zhang.
+
+Date : 2023.02.21
+*)
+
+From SLF (* TLC *) Require Export LibCore TLCbuffer.
+From SLF (* CBS *) Require Export Himpl.
+
+(* ################################################################# *)
+
+(*** Implicit Types (to improve the readability) ***)
+
+Implicit Types b bp : bloc.
+Implicit Types f fp: floc.
+Implicit Types ln : list int.
+Implicit Types n : int.
+Implicit Types v : val.
+Implicit Types t : trm.
+Implicit Types be : bool.
+Implicit Types hb : heapb.
+Implicit Types sb : stateb.
+Implicit Types hf : heapf.
+Implicit Types sf : statef.
+
+(*all operators have opaque definitions*)
+Global Opaque hbempty hbpure hbstar hbsingle hbexists hbforall.
+Global Opaque hfempty hfpure hfstar hfsingle hfexists hfforall.
+
+(* ################################################################# *)
+Open Scope liblist_scope.
+Open Scope Z_scope.
+
+(* ================================================================= *)
+(** ** Hoare reasoning rules ** **)
+
+(**============= * Definition of (total correctness) Hoare triples ================*)
+
+(* -- the behavior of trm in the entire state -- *)
+Definition hoare (t:trm) (H:hprop) (Q:val->hprop) :=
+forall sf sb, H (sf,sb) -> 
+  exists sf' sb' v, eval (sf,sb) t (sf',sb') v /\ Q v (sf',sb').
+
+(** ++++++++++++++++++++  Hoare Reasoning rules  ++++++++++++++++++++ **)
+
+(** ----- block prim operations ------- **)
+Lemma hoare_bcreate : forall Hf Hb ln,
+  hoare (bprim_create (val_listint ln))
+    (\R[ Hf, Hb])
+    (fun r => \exists b, \[r = val_bloc b] \* \R[ Hf, b ~b~> ln \b* Hb ]).
+Proof.
+  intros. intros sf sb K0.
+  destruct K0 as (P1&P2).
+  forwards~ (b&D&N): (Fmap.single_fresh 0%nat sb ln).
+  exists sf ((Fmap.single b ln) \u sb) (val_bloc b). subst.
+  simpls. splits~.
+  (*Notice!!*)
+  - applys~ eval_bcreate_sep.
+  - exists b. rewrite~ hstar_hpure.
+    splits~. splits~.
+    applys~ hbstar_intro.
+    applys~ hbsingle_intro.
+Qed.
+
+Lemma hoare_bget : forall Hf Hb b ln,
+  hoare (bprim_get (val_bloc b))
+    (\R[ Hf, ( (b ~b~> ln) \b* Hb) ])
+    ( fun r => \[r = (val_listint ln)] \* \R[ Hf, ((b ~b~> ln) \b* Hb)] ).
+Proof.
+  intros. intros sf sb K0.
+  destruct K0 as (P1&P2).
+  destruct P2 as (sb1&sb2&D1&D2&D3&D4).
+  exists sf sb (val_listint ln). subst.
+  splits~.
+  - lets (E1&N) : hbsingle_inv D1. subst. simpls.
+    applys~ eval_bget_sep. apply D4.
+  - rewrite~ hstar_hpure. splits~. splits~. simpls. substs~.
+    applys~ hbstar_intro.
+Qed.
+
+Lemma hoare_bdelete : forall Hf Hb b ln,
+  hoare (bprim_delete (val_bloc b))
+    (\R[ Hf, ( (b ~b~> ln) \b* Hb) ])
+    (fun r => \[r = val_unit] \* \R[ Hf, Hb ]).
+Proof.
+  intros. intros sf sb K0.
+  destruct K0 as (P1&P2).
+  destruct P2 as (sb1&sb2&D1&D2&D3&D4).
+  lets (E1&N): hbsingle_inv D1.
+  exists sf sb2 (val_unit). subst.
+  splits~.
+  - simpls. applys~ eval_bdelete_sep. apply D4.
+    apply D3.
+  - rewrite~ hstar_hpure. splits~. splits~.
+Qed.
+
+Lemma hoare_bappend : forall Hf Hb b ln1 ln2,
+  hoare (bprim_append (val_bloc b) (val_listint ln2))
+    ( \R[Hf, (b ~b~> ln1) \b* Hb] )
+    (fun _ => \R[Hf, (b ~b~> (ln1++ln2)) \b* Hb]).
+Proof.
+  intros. intros sf sb K.
+  destruct K as (K1&K2). simpls.
+  destruct K2 as (sb1&sb2&D1&D2&D3&D4).
+  lets (E1&N): hbsingle_inv D1.
+  subst.
+  exists sf (single b (ln1++ln2) \u sb2) val_unit.
+  splits.
+  - applys~ eval_bappend_sep.
+  - splits~. simpl.
+    applys~ hbstar_intro.
+      + applys~ hbsingle_intro.
+      + applys Fmap.disjoint_single_set D3.
+Qed.
+
+Lemma hoare_btruncate : forall Hf Hb b ln1 n,
+  hoare (bprim_trun (val_bloc b) n)
+    ( \R[Hf, (b ~b~> ln1) \b* Hb] )
+    (fun _ => \R[Hf, (b ~b~> (droplast (to_nat n) ln1)) \b* Hb]).
+Proof.
+  intros. intros sf sb K.
+  destruct K as (K1&K2). simpls.
+  destruct K2 as (sb1&sb2&D1&D2&D3&D4).
+  lets (E1&N): hbsingle_inv D1.
+  subst.
+  exists sf (single b (droplast (to_nat n) ln1) \u sb2) val_unit.
+  splits.
+  - applys~ eval_btruncate_sep.
+  - splits~. simpl.
+    applys~ hbstar_intro.
+      + applys~ hbsingle_intro.
+      + applys Fmap.disjoint_single_set D3.
+Qed.
+
+Lemma hoare_bsize : forall Hf Hb b ln1,
+  hoare (bprim_size (val_bloc b) )
+    ( \R[Hf, (b ~b~> ln1) \b* Hb] )
+    (fun r => \[r = List.length ln1] \* \R[Hf, (b ~b~> ln1) \b* Hb]).
+Proof.
+  intros. intros sf sb K.
+  destruct K as (K1&K2). simpls.
+  destruct K2 as (sb1&sb2&D1&D2&D3&D4).
+  exists sf sb (val_int (List.length ln1)).
+  lets (E1&N): hbsingle_inv D1. subst.
+  splits~.
+  applys~ eval_bsize_sep.
+  rewrite hstar_hpure_iff.
+  splits~. simpl.
+  splits~.
+  applys~ hbstar_intro.
+Qed.
+
+Lemma single_fresh_floc : forall hf lb,
+  exists f, Fmap.disjoint (single f lb) hf /\ f <> fnull.
+Proof using.
+  intros. forwards (f&F&N): exists_not_indom fnull hf.
+  exists f. split~. applys* disjoint_single_of_not_indom.
+Qed.
+
+(** ------------ file prim operations -------------- **)
+Lemma hoare_fcreate : forall Hf Hb lb,
+  hoare (fprim_create (val_listbloc lb))
+    (\R[ \f[] \f* Hf, Hb ])
+    (fun r => \exists f, (\[r = (val_floc f)] \* \R[ (f ~f~> lb) \f* Hf, Hb])).
+Proof.
+  intros. intros sf sb K0.
+  rewrite hfstar_hempty_l in K0.
+  destruct K0 as (KA&KB). simpls.
+  lets (f&D&N) : single_fresh_floc sf lb.
+  exists (Fmap.single f lb \u sf) sb (val_floc f). subst.
+  splits~.
+  - applys~ eval_fcreate_sep.
+  - exists f. rewrite~ hstar_hpure. splits~. splits~. simpls.
+    subst. applys~ hfstar_intro. applys~ hfsingle_intro.
+Qed.
+
+Lemma hoare_fget : forall Hf Hb f lb,
+  hoare (fprim_get (val_floc f))
+    (\R[ (f ~f~> lb \f* Hf), Hb])
+    (fun r => (\[r = val_listbloc lb]) \* \R[ ((f ~f~> lb) \f* Hf), Hb ]).
+Proof.
+  intros. intros sf sb ((sf1&sf2&D1&D2&D3&D4)&P2).
+  exists sf sb (val_listbloc lb). subst. simpls.
+  splits~.
+  - lets (E1&N) : hfsingle_inv D1. subst.
+    applys~ eval_fget_sep.
+  - rewrite hstar_hpure. splits~. splits~. simpls.
+    subst. applys~ hfstar_intro.
+Qed.
+
+Lemma hoare_fget_nth_blk : forall Hf Hb f lb n,
+  hoare (fprim_nthblk (val_floc f) n)
+    (\R[ (f ~f~> lb \f* Hf), Hb ])
+    (fun r => \[r = val_bloc (nth_default bnull (Z.to_nat n) lb)] \* \R[((f ~f~> lb) \f* Hf),Hb ]).
+Proof.
+  intros. intros sf sb K.
+  destruct K as (P1&P2).
+  destruct P1 as (sf1&sf2&D1&D2&D3&D4).
+  exists sf sb (val_bloc (nth_default bnull (Z.to_nat n) lb)). subst. simpls.
+  splits~.
+  - lets (E1&N) : hfsingle_inv D1. subst.
+    applys~ eval_fget_nth_blk_sep.
+  - rewrite hstar_hpure. splits~. splits~. subst. simpls.
+    applys~ hfstar_intro.
+Qed.
+
+Lemma hoare_fset_nth_blk : forall Hf Hb f lb n b,
+  hoare (fprim_set (val_floc f) n (val_bloc b))
+    (\R[ (f ~f~> lb \f* Hf), Hb ])
+    (fun r => \R[ ( (f ~f~> (LibList.update (to_nat n) b lb)) \f* Hf), Hb ]).
+Proof.
+  intros. intros sf sb K.
+  destruct K as (P1&P2).
+  destruct P1 as (sf1&sf2&D1&D2&D3&D4).
+  exists (single f (LibList.update (to_nat n) b lb) \u sf2) sb val_unit.
+  subst. simpls. lets (E1&N) : hfsingle_inv D1.
+  splits~.
+  - subst~.
+    applys~ eval_fset_nth_blk_sep.
+  - splits~.
+    applys~ hfstar_intro.
+      + applys~ hfsingle_intro.
+      + applys Fmap.disjoint_single_set.
+        rewrite~ <- E1.
+Qed.
+
+Lemma hoare_fdelete : forall Hf Hb f lb,
+  hoare (fprim_delete (val_floc f))
+    (\R[ (f ~f~> lb \f* Hf), Hb ])
+    (fun r => \[r = val_unit] \* \R[Hf, Hb]).
+Proof.
+  intros. intros sf sb K0.
+  destruct K0 as (P1&P2).
+  destruct P1 as (sf1&sf2&D1&D2&D3&D4).
+  lets (E1&N): hfsingle_inv D1.
+  exists sf2 sb val_unit. subst. simpls.
+  splits~.
+  - applys~ eval_fdelete_sep. apply D4. apply D3.
+  - rewrite hstar_hpure. splits~. splits~.
+Qed.
+
+Lemma hoare_fattach : forall Hf Hb f lb1 lb2,
+  hoare (fprim_attach (val_floc f) (val_listbloc lb2))
+    ( \R[(\f[] \f* (f ~f~> lb1) \f* Hf), Hb] )
+    (fun _ => \R[(f ~f~> (lb1++lb2)) \f* Hf, Hb]).
+Proof.
+  intros. intros sf sb K.
+  destruct K as (K1&K2). simpls.
+  rewrite hfstar_hempty_l in K1.
+  destruct K1 as (sf1&sf2&D1&D2&D3&D4).
+  lets (E1&N): hfsingle_inv D1.
+  subst.
+  exists (single f (lb1++lb2) \u sf2) sb val_unit.
+  splits.
+  - applys~ eval_fattach_sep.
+  - splits~. simpl.
+    applys~ hfstar_intro.
+      + applys~ hfsingle_intro.
+      + applys Fmap.disjoint_single_set D3.
+Qed.
+
+Lemma hoare_ftruncate : forall Hf Hb f lb n,
+  hoare (fprim_trun (val_floc f) n)
+    ( \R[(f ~f~> lb) \f* Hf, Hb] )
+    (fun _ => \R[(f ~f~> (droplast (to_nat n) lb)) \f* Hf, Hb]).
+Proof.
+  intros. intros sf sb K.
+  destruct K as (K1&K2). simpls.
+  destruct K1 as (sf1&sf2&D1&D2&D3&D4).
+  lets (E1&N): hfsingle_inv D1.
+  subst.
+  exists (single f (droplast (to_nat n) lb) \u sf2) sb val_unit.
+  splits.
+  - applys~ eval_ftruncate_sep.
+  - splits~. simpl.
+    applys~ hfstar_intro.
+      + applys~ hfsingle_intro.
+      + applys Fmap.disjoint_single_set D3.
+Qed.
+
+Lemma hoare_fsize : forall Hf Hb f lb,
+  hoare (fprim_size (val_floc f) )
+    ( \R[(f ~f~> lb) \f* Hf, Hb] )
+    (fun r => \[r = List.length lb] \* \R[(f ~f~> lb) \f* Hf, Hb]).
+Proof.
+  intros. intros sf sb K.
+  destruct K as (K1&K2). simpls.
+  destruct K1 as (sf1&sf2&D1&D2&D3&D4).
+  exists sf sb (val_int (List.length lb)).
+  lets (E1&N): hfsingle_inv D1. subst.
+  splits~. applys~ eval_fsize_sep.
+  rewrite hstar_hpure_iff.
+  splits~. splits~.
+  applys~ hfstar_intro.
+Qed.
+
+(** -------- aux prim operation  ----------- **)
+Lemma hoare_add : forall H n1 n2,
+  hoare (val_add n1 n2) H
+    (fun r => (\[r = (n1+n2)] \* H)).
+Proof.
+  intros. intros sf sb.
+  intros M.
+  exists sf sb (n1+n2). splits.
+  apply eval_add.
+  applys* hstar_hpure_iff.
+Qed.
+
+Lemma hoare_min : forall H n1 n2,
+  hoare (val_min n1 n2) H
+    (fun r => (\[r = (n1-n2)] \* H)).
+Proof.
+  intros. intros sf sb.
+  intros M.
+  exists sf sb (n1-n2). splits.
+  apply eval_min.
+  applys* hstar_hpure_iff.
+Qed.
+
+Lemma hoare_le : forall H n1 n2,
+  hoare (val_le n1 n2) H
+    (fun r => (\[r = (val_bool (isTrue (n1 <= n2)))] \* H)).
+Proof.
+  intros. intros sf sb.
+  intros M.
+  exists sf sb (val_bool (isTrue (n1 <= n2))). splits.
+  apply eval_le.
+  applys* hstar_hpure_iff.
+Qed.
+
+Lemma hoare_eq : forall H n1 n2,
+  hoare (val_eq n1 n2) H
+    (fun r => (\[r = val_bool (n1 =? n2)] \* H)).
+Proof.
+  intros. intros sf sb.
+  intros M.
+  exists sf sb (val_bool (n1 =? n2)). splits.
+  apply eval_eq.
+  applys* hstar_hpure_iff.
+Qed.
+
+Lemma hoare_list_rev : forall H ln1,
+  hoare (val_list_rev (val_listint ln1)) H
+    (fun r => (\[r = val_listint (rev ln1)] \* H)).
+Proof.
+  intros. intros sf sb.
+  intros M.
+  exists sf sb (val_listint (rev ln1)). splits.
+  apply eval_list_rev.
+  applys* hstar_hpure_iff.
+Qed.
+
+Lemma hoare_list_app : forall H ln1 ln2,
+  hoare (val_list_app (val_listint ln1) (val_listint ln2)) H
+    (fun r => (\[r = val_listint (ln1 ++ ln2)] \* H)).
+Proof.
+  intros. intros sf sb.
+  intros M.
+  exists sf sb (val_listint (ln1 ++ ln2)). splits.
+  apply eval_list_app.
+  applys* hstar_hpure_iff.
+Qed.
+
+
+(** --------- terms  ---------**)
+Lemma hoare_eval_like : forall t1 t2 H Q,
+  eval_like t1 t2 ->
+  hoare t1 H Q ->
+  hoare t2 H Q.
+Proof.
+  introv E M1 K0. forwards (sf'&sb'&v&R1&K1) : M1 K0.
+  exists sf' sb' v. splits~.
+Qed.
+
+Lemma hoare_val : forall v H Q,
+  H ==> Q v ->
+  hoare (trm_val v) H Q.
+Proof.
+  introv M. intros hf hb k.
+  exists hf hb v. splits~.
+  applys eval_val.
+Qed.
+
+Lemma hoare_fun : forall x t1 H Q,
+  H ==> Q (val_fun x t1) ->
+  hoare (trm_fun x t1) H Q.
+Proof.
+  introv M. intros hf hb k. exists hf hb __.
+  splits~. applys eval_fun.
+Qed.
+
+Lemma hoare_fix : forall F x t1 H Q,
+  H ==> Q (val_fix F x t1) ->
+  hoare (trm_fix F x t1) H Q.
+Proof.
+  introv M. intros hf hb k. exists hf hb __.
+  splits~. apply eval_fix.
+Qed.
+
+Lemma hoare_app_fun: forall v1 v2 x t1 H Q,
+  v1 = val_fun x t1 ->
+  hoare (subst x v2 t1) H Q ->
+  hoare (trm_app v1 v2) H Q.
+Proof.
+  introv E M. intros sf sb K0.
+  forwards (sf'&sb'&v&R1&K1) : (rm M) K0.
+  exists sf' sb' v.
+  splits~. applys eval_app_fun E R1.
+Qed.
+
+Lemma hoare_app_fix:forall v1 v2 F x t1 H Q,
+  v1 = val_fix F x t1 ->
+  hoare (subst x v2 (subst F v1 t1)) H Q ->
+  hoare (trm_app v1 v2) H Q.
+Proof.
+  introv E M. intros sf sb K0. forwards (sf'&sb'&v&R1&K1): (rm M) K0.
+  exists sf' sb' v. splits. { applys eval_app_fix E R1. } { applys K1. }
+Qed.
+
+Lemma hoare_seq : forall t1 t2 H Q H1,
+  hoare t1 H (fun r => H1) ->
+  hoare t2 H1 Q ->
+  hoare (trm_seq t1 t2) H Q.
+Proof using.
+  introv M1 M2 Hh.
+  forwards* (hf1&hb1&v1&R1&K1): (rm M1).
+  forwards* (hf2&hb2&v2&R2&K2): (rm M2).
+  exists hf2 hb2 v2. splits~. { applys~ eval_seq R1 R2. }
+Qed.
+
+Lemma hoare_let : forall x t1 t2 H Q Q1,
+  hoare t1 H Q1 ->
+  (forall v, hoare (subst x v t2) (Q1 v) Q) ->
+  hoare (trm_let x t1 t2) H Q.
+Proof using.
+  introv M1 M2 Hh.
+  forwards* (hf1&hb1&v1&R1&K1): (rm M1).
+  forwards* (hf2&hb2&v2&R2&K2): (rm M2).
+  exists hf2 hb2 v2. splits~. { applys~ eval_let R2. }
+Qed.
+
+Lemma hoare_if : forall (be:bool) t1 t2 H Q,
+  hoare (if be then t1 else t2) H Q ->
+  hoare (trm_if be t1 t2) H Q.
+Proof using.
+  introv M1. intros hf hb Hh. forwards* (hf1&hb1&v1&R1&K1): (rm M1).
+  exists hf1 hb1 v1. splits~. { applys* eval_if. }
+Qed.
+
+(*----- structural rules ------*)
+Lemma hoare_conseq : forall t H' Q' H Q,
+  hoare t H' Q' ->
+  H ==> H' ->
+  Q' ===> Q ->
+  hoare t H Q.
+Proof using.
+  introv M MH MQ HF. forwards (sf'&sb'&v&R&K): M sf sb. { applys~ himpl_inv. }
+  exists sf' sb' v. splits~. { applys~ himpl_inv. }
+Qed.
+
+
+(* ================================================================================ *)
