Removedup.v
@@ -1,0 +1,126 @@
+From SLF (* TLC *) Require Export LibCore.
+From SLF (* Sep *) Require Export TLCbuffer Var Fmap Language.
+(**===================== List Function for MapReduce =============================**)
+
+Definition bloc : Type := nat.
+Definition floc : Type := nat.
+
+(* wordcount kvpair (word, times) *)
+Definition wdpair : Type := int * int.
+
+(* =================== For WordCount ==================== *)
+
+(*-- compare kvpair --*)
+Definition eqword (p1 p2: wdpair) := (fst p1) =? (fst p2).
+
+Definition neqword (p1 p2: wdpair) := negb (eqword p1 p2).
+
+(*--  reflexivity  --*)
+Lemma eqword_refl : forall a,
+  eqword a a = true.
+Proof. intros. unfold eqword. simpl. apply~ Z.eqb_eq. Qed.
+
+Lemma neqword_refl : forall a,
+  neqword a a = false.
+Proof. intros. unfold neqword. rewrite~ eqword_refl. Qed.
+
+
+(*-- remove function is similar to filter  --*)
+Lemma filter_nil : forall (a:wdpair),
+  List.filter (neqword a) nil = nil.
+Proof using. auto. Qed.
+
+Lemma filter_cons : forall a x l,
+  List.filter (neqword a) (x::l) = 
+(If (neqword a) x then
+ x :: List.filter (neqword a) l else List.filter (neqword a) l).
+Proof using.
+  intros. simpl. case_if; symmetry.
+  apply~ If_l. apply~ If_r.
+Qed.
+
+Lemma filter_eq_self_of_mem_implies : forall l a,
+  (forall x, mem x l -> ((neqword a) x)) ->
+  List.filter (neqword a) l = l.
+Proof using.
+  induction l; introv M.
+  { auto. }
+  { rewrite filter_cons. case_if.
+    { fequals. applys IHl. introv Mx. applys* M. }
+    { false* M. } }
+Qed.
+
+Lemma mem_filter_eq : forall (x a:wdpair) (l:list wdpair),
+  mem x (List.filter (neqword a) l) = 
+(mem x l /\ (neqword a) x).
+Proof using.
+  intros. extens. induction l.
+  { rewrite filter_nil. iff M (M&?); inverts M. }
+  { rewrite filter_cons. case_if; rew_listx; rewrite IHl.
+    { iff [M|M] N; subst*. }
+    { iff M ([N|N]&K); subst*. } }
+Qed.
+
+Lemma noduplicates_filter : forall (a:wdpair) (l:list wdpair),
+  noduplicates l ->
+  noduplicates (List.filter (neqword a) l).
+Proof using.
+  introv H. induction H.
+  simpl. apply noduplicates_nil.
+  simpl. case_if*.
+  rewrite <- app_cons_one_r.
+  apply noduplicates_app.
+  apply noduplicates_one.
+  auto.
+  intros. apply H.
+  rewrite mem_filter_eq in H2.
+  destruct H2 as (H2a&H2b).
+  rewrite mem_cons_eq in H1.
+  destruct H1. subst~.
+  rewrite mem_nil_eq in H1. destruct H1.
+Qed.
+
+(* remove as filter *)
+Lemma remove_as_filter : forall a l,
+  remove a l = List.filter (neqword a) l.
+Proof using. auto. Qed.
+
+(* no duplicate elements before removal, and none after *)
+Lemma noduplicates_remove : forall a l,
+  noduplicates l ->
+  noduplicates (remove a l).
+Proof using.
+  intros. rewrite remove_as_filter. applys* noduplicates_filter.
+Qed.
+
+Lemma mem_remove_eq : forall x a l,
+  mem x (remove a l) = (mem x l /\ (neqword a x)).
+Proof using. intros. applys* mem_filter_eq. Qed.
+
+
+(*=========== the sequence after removal has no duplicate elements =============*)
+Lemma remove_duplicates_spec : forall l l',
+  l' = remove_duplicates l -> noduplicates l'.
+Proof using.
+  introv E.
+  gen l' E. induction l; introv E; simpls.
+    { subst. apply noduplicates_nil. }
+    { sets_eq l'': (remove_duplicates l).
+      rewrite E.
+      rewrite <- app_cons_one_r.
+      apply noduplicates_app.
+      apply noduplicates_one.
+      auto. applys noduplicates_remove. apply~ IHl.
+      intros. rewrite mem_remove_eq in H0.
+      destruct H0 as (H1&H2).
+      rewrite mem_cons_eq in H.
+  destruct H. subst x. 
+  rewrite neqword_refl in H2.
+  auto. rewrite mem_nil_eq in H. destruct H. }
+Qed.
+
+Lemma noduplicates_remove_duplicates : forall l,
+  noduplicates (remove_duplicates l).
+Proof.
+  intros. applys* remove_duplicates_spec.
+Qed.
