TripleAndRules.v
@@ -1,0 +1,1024 @@
+(** 
+This file describes the construction of our proof system, mainly about:
+  1. The definitions of Separation Logic triple in CBS:
+    a. three different definitions of CBS-SL-triple
+    b. prove the equivalence of three definitions
+  2. how to state and prove the reasoning rules of:
+    a. primitive operations (block & file)
+    b. terms
+    c. structural rules
+  (we can prove the SL rules by the proven Hoare rules ).
+
+Author: Bowen Zhang.
+
+Date : 2023.02.22
+*)
+
+From SLF (* TLC *) Require Export LibCore TLCbuffer.
+From SLF (* CBS *) Require Export Himpl Hoare.
+
+(* ################################################################# *)
+
+(*** Implicit Types (to improve the readability) ***)
+
+Implicit Types b bp : bloc.
+Implicit Types f fp: floc.
+Implicit Types ln : list int.
+Implicit Types n : int.
+Implicit Types v : val.
+Implicit Types t : trm.
+Implicit Types be : bool.
+Implicit Types hb : heapb.
+Implicit Types sb : stateb.
+Implicit Types hf : heapf.
+Implicit Types sf : statef.
+
+(*all operators have opaque definitions*)
+Global Opaque hbempty hbpure hbstar hbsingle hbexists hbforall.
+Global Opaque hfempty hfpure hfstar hfsingle hfexists hfforall.
+
+(* ################################################################# *)
+Open Scope liblist_scope.
+Open Scope Z_scope.
+
+(* ================================================================================ *)
+(** ** Separation Logic Formal System for CBS ** **)
+
+(**============= * Definition of Separation Logic triple ================*)
+(* 1st way: using refinement predicate *)
+Definition triple (t:trm) (H:hprop) (Q:val->hprop) : Prop :=
+forall Hf Hb,
+    hoare t (H \* \R[Hf,Hb]) (Q \*+ \R[Hf,Hb]).
+
+(* 2nd way: using CBS predicate *)
+Definition triple_pred (t:trm) (H:hprop) (Q:val->hprop) : Prop :=
+forall H',
+    hoare t (H \* H') (Q \*+ H').
+
+(* 3rd way: using CBS heap *)
+Definition triple_lowlevel (t:trm) (H:hprop) (Q:val->hprop) : Prop :=
+forall h1 h2,
+  glodisjoint h1 h2 ->
+  H h1 ->
+  exists h1' v,
+       glodisjoint h1' h2
+    /\ eval (h1 \g h2) t (h1' \g h2) v
+    /\ Q v h1'.
+
+(* 1st definition <-> 2nd definition *)
+Definition triple_iff_triple_pred: forall t H Q,
+  triple_pred t H Q  <->  triple t H Q.
+Proof.
+  intros. unfolds~ triple_pred,triple. iff* R.
+  intros H'. lets M : refine_eq' H'. rewrite M.
+  intros hf hb (h1&h2&KA&(hf1&hb1&h11&h12&KB1&KB2&KB3&KB4)&KC&KD).
+  lets T : R (= hf1) (= hb1) hf hb.
+  apply hpure_inv in KB1 as (KB11&KB12).
+  subst. unfold glounion in KD.
+  simpls. do 2 rewrite union_empty_l in KD.
+  lets C : hstar_intro KA KB2 KC.
+  unfold glounion in C. rewrite <- KD in C.
+  apply T in C as (hf'&hb'&v&CA&CB).
+  exists hf' hb' v. splits~.
+  destruct CB as (h3&h4&C1&C2&C3&C4).
+  exists~ h3 h4. splits~.
+  exists~ hf1 hb1. rewrite hstar_hpure_iff.
+  splits~.
+Qed.
+
+(* 2nd definition <-> 3rd definition *)
+Lemma triple_pred_iff_triple_lowlevel : forall t H Q,
+  triple_pred t H Q <-> triple_lowlevel t H Q.
+Proof using.
+  unfold triple_pred,triple_lowlevel. iff* M.
+  - introv D P1. unfold hoare in M.
+    forwards~ (hf'&hb'&v&R1&R2):
+      (rm M) (=h2) ((fst h1) \u (fst h2)) ((snd h1) \u (snd h2)).
+    exists~ h1 h2.
+    destruct R2 as (h1'&h2'&HA&HB&HC&HD).
+    subst. exists~ h1' v. splits~.
+    rewrite HD in R1. apply R1.
+  - introv (h1&h2&HA&HB&HC&HD).
+    forwards* (h1'&v&MC&MD&ME) : (rm M) h1 h2.
+    exists ((fst h1') \u (fst h2)) ((snd h1') \u (snd h2)) v.
+    rewrite HD. split~.  apply* hstar_intro.
+Qed.
+
+(**====================  separation logic rule  ===========================**)
+
+(*------------------ SL rule: block prim operations---------------*)
+Lemma triple_bcreate : forall Hf ln,
+  triple (bprim_create (val_listint ln))
+    (\R[ Hf, \b[] ])
+    (fun r => \exists b, \[r= (val_bloc b)] \* (\R[ Hf, (b ~b~> ln)]) ).
+Proof.
+  intros. unfold triple. intros Hf' Hb'.
+  applys hoare_conseq hoare_bcreate hstar_sep_l.
+
+  intros r h M.
+  destruct M as (b&M).
+  apply hstar_hpure_iff in M as [M1 M].
+  destruct M as (MA&MB). 
+  rewrite hstar_hexists. exists b.
+  rewrite hstar_assoc, hstar_hpure. splits~.
+  rewrite hstar_sep, state_get_eq.
+  splits~. simpls.
+  rewrite hbstar_hempty_l in MB. auto.
+Qed.
+
+Lemma triple_bget: forall Hf b ln,
+  triple (bprim_get b)
+    (\R[ Hf, (b ~b~> ln)])
+    (fun r => \[r=(val_listint ln)] \* (\R[ Hf, (b ~b~> ln)])).
+Proof.
+  intros. unfold triple. intros Hf' Hb'.
+  applys hoare_conseq hoare_bget hstar_sep_l.
+  intros r h R.
+  apply hstar_hpure_iff in R as [R1 R].
+  destruct R as (HA&HB).
+  rewrite hstar_assoc, hstar_hpure. splits~.
+  rewrite hstar_sep, state_get_eq.
+  splits~.
+Qed.
+
+Lemma triple_bdelete: forall Hf b ln,
+  triple (bprim_delete b)
+    (\R[ Hf, (b ~b~> ln)])
+    (fun _ =>(\R[ Hf, \b[]])).
+Proof.
+  intros. unfold triple. intros Hf' Hb'.
+  applys hoare_conseq hoare_bdelete hstar_sep_l.
+  intros r h R.
+  apply hstar_hpure_iff in R as [R1 R].
+  destruct R as (HA&HB).
+  rewrite hstar_sep, state_get_eq.
+  splits~. simpls. rewrite~ hbstar_hempty_l.
+Qed.
+
+Lemma triple_bappend : forall Hf b ln1 ln2,
+  triple (bprim_append b (val_listint ln2))
+    ( \R[Hf, (b ~b~> ln1)] )
+    (fun _ => \R[Hf, b ~b~> (ln1++ln2)]).
+Proof.
+  intros. unfold triple. intros Hf' Hb'.
+  applys hoare_conseq hoare_bappend.
+  rewrite hstar_sep. apply himpl_refl.
+  intros r h (RA&RB).
+  rewrite hstar_sep, state_get_eq.
+  splits~.
+Qed.
+
+Lemma triple_btruncate : forall Hf b l n,
+  triple (bprim_trun b n)
+    ( \R[Hf, (b ~b~> l)] )
+    (fun _ => \R[Hf, b ~b~> (droplast (to_nat n) l)]).
+Proof.
+  intros. unfold triple. intros Hf' Hb'.
+  applys hoare_conseq hoare_btruncate.
+  rewrite hstar_sep. apply himpl_refl.
+  intros r h (RA&RB).
+  rewrite hstar_sep, state_get_eq.
+  splits~.
+Qed.
+
+Lemma triple_bsize : forall Hf b ln1,
+  triple (bprim_size b )
+    ( \R[Hf, (b ~b~> ln1)] )
+    (fun r => \[r = List.length ln1] \* \R[Hf, (b ~b~> ln1)]).
+Proof.
+  intros. unfold triple. intros Hf' Hb'.
+  applys hoare_conseq hoare_bsize.
+  rewrite hstar_sep. apply himpl_refl.
+  intros r h R.
+  rewrite hstar_hpure_iff in R.
+  destruct R as (RA&RB).
+  rewrite hstar_assoc. rewrite hstar_hpure.
+  splits~. rewrite~ hstar_sep.
+Qed.
+
+(*-------------------- SL rule: file prim operations -------------------*)
+Lemma triple_fcreate : forall Hb lb,
+  triple (fprim_create (val_listbloc lb))
+    (\R[ \f[], Hb ])
+    (fun r => \exists f, \[r = val_floc f] \* \R[(f ~f~> lb), Hb ]).
+Proof.
+  intros. intros Hf' Hb'.
+  applys hoare_conseq hoare_fcreate hstar_sep_l.
+  introv (f&M).
+  apply hstar_hpure_iff in M as (M1&(MA&MB)).
+  rewrite hstar_hexists. exists f.
+  rewrite hstar_assoc, hstar_hpure. splits~.
+  rewrite hstar_sep. splits~.
+Qed.
+
+Lemma triple_fget: forall Hb (f:floc) lb,
+  triple (fprim_get f)
+    (\R[ (f ~f~> lb), Hb])
+    (fun r =>\[r=(val_listbloc lb)] \* \R[(f ~f~> lb), Hb]).
+Proof.
+  intros. intros Hf' Hb'.
+  applys hoare_conseq hoare_fget hstar_sep_l.
+  intros r h M.
+  apply hstar_hpure_iff in M as (MA&(M1&M2)).
+  rewrite hstar_assoc, hstar_hpure. splits~.
+  rewrite hstar_sep. splits~.
+Qed.
+
+Lemma triple_fget_nth_blk : forall Hb f lb n,
+  triple (fprim_nthblk f n)
+    (\R[ f ~f~> lb, Hb ])
+    (fun r => \[r = val_bloc (nth_default bnull (Z.to_nat n) lb)] \* 
+              \R[(f ~f~> lb),Hb ]).
+Proof.
+  intros. intros Hf' Hb'.
+  applys hoare_conseq hoare_fget_nth_blk hstar_sep_l.
+  intros r h M.
+  apply hstar_hpure_iff in M as [MA M].
+  destruct M as (M1&M2).
+  rewrite hstar_assoc, hstar_hpure. splits~.
+  rewrite hstar_sep, state_get_eq. splits~.
+Qed.
+
+Lemma triple_fset_nth_blk : forall Hb f lb n b,
+  triple (fprim_set f n b)
+    (\R[ f ~f~> lb, Hb ])
+    (fun r => \R[ (f ~f~> (LibList.update (Z.to_nat n) b lb)), Hb ]).
+Proof.
+  intros. intros Hf' Hb'.
+  applys hoare_conseq hoare_fset_nth_blk hstar_sep_l.
+  intros r h M.
+  destruct M as (M1&M2).
+  rewrite hstar_sep, state_get_eq.
+  splits~.
+Qed.
+
+Lemma triple_fdelete: forall Hb f lb,
+  triple (fprim_delete f)
+    (\R[ (f ~f~> lb), Hb])
+    (fun r =>(\R[ \f[], Hb])).
+Proof.
+  intros. intros Hf' Hb'.
+  applys hoare_conseq hoare_fdelete hstar_sep_l.
+  intros r h M.
+  apply hstar_hpure_iff in M as [MA M].
+  destruct M as (M1&M2).
+  rewrite hstar_sep, state_get_eq.
+  splits~. simpl.
+  rewrite~ hfstar_hempty_l.
+Qed.
+
+Lemma triple_fattach: forall Hb f lb1 lb2,
+  triple (fprim_attach f (val_listbloc lb2))
+    ( \R[(f ~f~> lb1), Hb] )
+    (fun r =>(\R[(f ~f~> (lb1++lb2)), Hb])).
+Proof.
+  intros. intros Hf' Hb'.
+  applys hoare_conseq hoare_fattach.
+  rewrite hstar_sep, hfstar_hempty_l.
+  apply himpl_refl.
+  intros r. rewrite hstar_sep. apply himpl_refl.
+Qed.
+
+Lemma triple_ftrun : forall Hb f lb n,
+  triple (fprim_trun f n)
+    ( \R[ (f ~f~> lb), Hb] )
+    (fun _ => \R[f ~f~> (droplast (to_nat n) lb), Hb]).
+Proof.
+  intros. unfold triple. intros Hf' Hb'.
+  applys hoare_conseq hoare_ftruncate.
+  rewrite hstar_sep. apply himpl_refl.
+  intros r h (RA&RB).
+  rewrite hstar_sep, state_get_eq.
+  splits~.
+Qed.
+
+Lemma triple_fsize : forall Hb f lb,
+  triple (fprim_size f )
+    ( \R[(f ~f~> lb), Hb] )
+    (fun r => \[r = List.length lb] \* \R[(f ~f~> lb), Hb]).
+Proof.
+  intros. unfold triple. intros Hf' Hb'.
+  applys hoare_conseq hoare_fsize.
+  rewrite hstar_sep. apply himpl_refl.
+  intros r h R.
+  rewrite hstar_hpure_iff in R.
+  destruct R as (RA&RB).
+  rewrite hstar_assoc. rewrite hstar_hpure.
+  splits~. rewrite~ hstar_sep.
+Qed.
+
+
+(* -------------------- SL rule: aux prim operations------------------ *)
+
+Lemma triple_add : forall H n1 n2,
+  triple (val_add n1 n2) H
+    (fun r => (\[r = (n1 + n2)] \* H)).
+Proof.
+  intros. unfold triple. intros Hf Hb sf sb M.
+  exists sf sb (n1+n2).
+  splits~. apply eval_add.
+  rewrite hstar_assoc.
+  apply* hstar_hpure_iff.
+Qed.
+
+Lemma triple_min : forall H n1 n2,
+  triple (val_min n1 n2) H
+    (fun r => (\[r = (n1 - n2)] \* H)).
+Proof.
+  intros. unfold triple. intros Hf Hb sf sb M.
+  exists sf sb (n1-n2).
+  splits~. apply eval_min.
+  rewrite hstar_assoc.
+  apply* hstar_hpure_iff.
+Qed.
+
+Lemma triple_eq : forall H n1 n2,
+  triple (val_eq n1 n2) H
+    (fun r => (\[r = val_bool (n1 =? n2)] \* H)).
+Proof.
+  intros. unfold triple. intros Hf Hb sf sb M.
+  exists sf sb (val_bool (n1 =? n2)).
+  splits~. apply eval_eq.
+  rewrite hstar_assoc.
+  apply* hstar_hpure_iff.
+Qed.
+
+Lemma triple_le : forall H n1 n2,
+  triple (val_le n1 n2) H
+    (fun r => (\[r = (val_bool (isTrue (n1 <= n2)))] \* H)).
+Proof.
+  intros. unfold triple. intros Hf Hb sf sb M.
+  exists sf sb (val_bool (isTrue (n1 <= n2))). splits.
+  apply eval_le.
+  rewrite hstar_assoc.
+  apply* hstar_hpure_iff.
+Qed.
+
+Lemma triple_list_rev : forall H ln1,
+  triple (val_list_rev (val_listint ln1)) H
+    (fun r => (\[r = val_listint (rev ln1)] \* H)).
+Proof.
+  intros. unfold triple. intros Hf Hb sf sb M.
+  exists sf sb (val_listint (rev ln1)).
+  splits~. apply eval_list_rev.
+  rewrite hstar_assoc.
+  apply* hstar_hpure_iff.
+Qed.
+
+Lemma triple_list_app : forall H ln1 ln2,
+  triple (val_list_app (val_listint ln1) (val_listint ln2)) H
+    (fun r => (\[r = val_listint (ln1 ++ ln2)] \* H)).
+Proof.
+  intros. intros Hf Hb sf sb M.
+  exists sf sb (val_listint (ln1 ++ ln2)). splits.
+  apply eval_list_app. rewrite hstar_assoc.
+  applys* hstar_hpure_iff.
+Qed.
+
+Lemma triple_blist_rev : forall H lb,
+  triple (val_blist_rev (val_listbloc lb))
+    H
+    ( fun r => \[r = (val_listbloc (rev lb))] \* H ).
+Proof.
+  intros. intros Hf Hb sf sb M.
+  exists sf sb (val_listbloc (rev lb)). splits.
+  apply eval_blist_rev. rewrite hstar_assoc.
+  applys* hstar_hpure_iff.
+Qed.
+
+Lemma triple_new_buffer : forall b H,
+  triple (val_new_blist b)
+    H
+    (fun r => \[r= val_listbloc (b::nil)] \* H ).
+Proof.
+  intros. intros Hf Hb sf sb M.
+  exists sf sb (val_listbloc (b::nil)). splits.
+  apply eval_new_blist. rewrite hstar_assoc.
+  applys* hstar_hpure_iff.
+Qed.
+
+Lemma triple_blist_buffer : forall b lb H,
+  triple (val_blist_buffer b (val_listbloc lb))
+    H
+    ( fun r => \[r = (val_listbloc (b::lb))] \* H ).
+Proof.
+  intros. intros Hf Hb sf sb M.
+  exists sf sb (val_listbloc (b::lb)). splits.
+  apply eval_blist_buffer. rewrite hstar_assoc.
+  applys* hstar_hpure_iff.
+Qed.
+
+Lemma triple_list_hd_bk : forall H ln1,
+  triple (val_list_hd_bk (val_listint ln1)) H
+    (fun r => (\[r = val_listint (take 2%nat ln1)] \* H)).
+Proof.
+  intros. unfold triple. intros Hf Hb sf sb M.
+  exists sf sb (val_listint (take 2%nat ln1)).
+  splits~. apply eval_list_hd_blk.
+  rewrite hstar_assoc.
+  apply* hstar_hpure_iff.
+Qed.
+
+Lemma triple_list_tl_bk : forall H ln1,
+  triple (val_list_tl_bk (val_listint ln1)) H
+    (fun r => (\[r = val_listint (drop 2%nat ln1)] \* H)).
+Proof.
+  intros. unfold triple. intros Hf Hb sf sb M.
+  exists sf sb (val_listint (drop 2%nat ln1)).
+  splits~. apply eval_list_tl_blk.
+  rewrite hstar_assoc.
+  apply* hstar_hpure_iff.
+Qed.
+
+
+Lemma triple_list_hd : forall H ln1,
+  triple (val_list_hd (val_listint ln1)) H
+    (fun r => (\[r = val_listint (take 1%nat ln1)] \* H)).
+Proof.
+  intros. unfold triple. intros Hf Hb sf sb M.
+  exists sf sb (val_listint (take 1%nat ln1)).
+  splits~. apply eval_list_hd.
+  rewrite hstar_assoc.
+  apply* hstar_hpure_iff.
+Qed.
+
+Lemma triple_list_tl : forall H ln1,
+  triple (val_list_tl (val_listint ln1)) H
+    (fun r => (\[r = val_listint (drop 1%nat ln1)] \* H)).
+Proof.
+  intros. unfold triple. intros Hf Hb sf sb M.
+  exists sf sb (val_listint (drop 1%nat ln1)).
+  splits~. apply eval_list_tl.
+  rewrite hstar_assoc.
+  apply* hstar_hpure_iff.
+Qed.
+
+Lemma triple_list_len : forall H ln1,
+  triple (val_list_len (val_listint ln1)) H
+    (fun r => (\[r = (LibList.length ln1)] \* H)).
+Proof.
+  intros. unfold triple. intros Hf Hb sf sb M.
+  exists sf sb (LibList.length ln1).
+  splits~. apply eval_list_len.
+  rewrite hstar_assoc.
+  apply* hstar_hpure_iff.
+Qed.
+
+(* ----------------  SL rule: terms   --------------- *)
+Lemma triple_val : forall v H Q,
+  H ==> Q v ->
+  triple (trm_val v) H Q.
+Proof.
+  introv M. unfold triple. intros. applys hoare_val.
+  applys~ himpl_frame_l.
+Qed.
+
+Lemma triple_val' : forall v H,
+  triple (trm_val v) H (fun r => \[r = v] \* H).
+Proof.
+  introv M. unfold triple. intros.
+  exists sf sb v. splits~. apply eval_val.
+  rewrite hstar_assoc, hstar_hpure_iff.
+  splits~.
+Qed.
+
+Lemma triple_fix: forall F x t1 H Q,
+  H ==> Q (val_fix F x t1) ->
+  triple (trm_fix F x t1) H Q.
+Proof.
+  unfold triple. introv M.
+  intros Hf' Hb' hf hb K.
+  exists hf hb __.
+  splits~. apply eval_fix.
+  eapply himpl_frame_l in M.
+  applys M K.
+Qed.
+
+Lemma triple_eval_like : forall t1 t2 H Q,
+  eval_like t1 t2 ->
+  triple t1 H Q ->
+  triple t2 H Q.
+Proof using.
+  introv E M1. intros Hf Hb. applys hoare_eval_like E. applys M1.
+Qed.
+
+Lemma triple_trm_equiv : forall t1 t2 H Q,
+  trm_equiv t1 t2 ->
+  triple t1 H Q <-> triple t2 H Q.
+Proof using.
+  introv E. unfolds trm_equiv. iff M.
+  { applys triple_eval_like M. introv R. applys* E. }
+  { applys triple_eval_like M. introv R. applys* E. }
+Qed.
+
+Lemma triple_fun : forall x t1 H Q,
+  H ==> Q (val_fun x t1) ->
+  triple (trm_fun x t1) H Q.
+Proof.
+  introv M.
+  unfold triple. intros Hf Hb hf hb K.  
+  exists hf hb __. splits~. applys eval_fun.
+  eapply himpl_frame_l in M.
+  applys M K.
+Qed.
+
+Lemma triple_app_fun : forall x v1 v2 t1 H Q,
+  v1 = val_fun x t1 ->
+  triple (subst x v2 t1) H Q ->
+  triple (trm_app v1 v2) H Q.
+Proof.
+  introv M N.
+  applys triple_eval_like N.
+  introv R. applys eval_app_fun M R.
+Qed.
+
+Lemma triple_app_fix : forall v1 v2 F x t1 H Q,
+  v1 = val_fix F x t1 ->
+  triple (subst x v2 (subst F v1 t1)) H Q ->
+  triple (trm_app v1 v2) H Q.
+Proof.
+  introv M N.
+  applys triple_eval_like N.
+  introv R. applys eval_app_fix M R.
+Qed.
+
+Lemma triple_seq : forall t1 t2 H Q H1,
+  triple t1 H (fun v => H1) ->
+  triple t2 H1 Q ->
+  triple (trm_seq t1 t2) H Q.
+Proof.
+  introv M1 M2. intros Hf Hb hf hb M.
+  forwards* (hf1&hb1&v1&R1&K1): (rm M1).
+  forwards* (hf2&hb2&v2&R2&K2): (rm M2).
+  exists hf2 hb2 v2. splits~. { applys~ eval_seq R1 R2. }
+Qed.
+
+Lemma triple_let :forall x t1 t2 H Q Q1,
+  triple t1 H Q1 ->
+  (forall v, triple (subst x v t2) (Q1 v) Q) ->
+  triple (trm_let x t1 t2) H Q.
+Proof.
+  introv M1 M2. intros Hf Hb hf hb M.
+  forwards* (hf1&hb1&v1&R1&K1): (rm M1).
+  forwards* (hf2&hb2&v2&R2&K2): (rm M2).
+  exists hf2 hb2 v2. splits~. { applys~ eval_let R2. }
+Qed.
+
+Lemma triple_if : forall be t1 t2 H Q,
+  triple (if be then t1 else t2) H Q ->
+  triple (trm_if (val_bool be) t1 t2) H Q.
+Proof.
+  introv M. intros Hf Hb hf hb K.
+  forwards* (hf1&hb1&v1&R1&K1): (rm M).
+  exists hf1 hb1 v1. splits~. { applys* eval_if. }
+Qed.
+
+
+(* ------------ SL structural rules ----------------- *)
+
+(*  _______________Frame Rule in CBS__________________  *)
+Lemma triple_frame : forall t H Q Hf Hb,
+  triple t H Q ->
+  triple t (H \* (\R[Hf,Hb])) (Q \*+ (\R[Hf,Hb])).
+Proof.
+  unfold triple, hoare. introv M.
+  intros Hf' Hb' sf sb.
+  specializes M (Hf \f* Hf') (Hb \b* Hb'). introv N.
+  rewrite hstar_assoc, hstar_sep in N.
+  apply M in N as (sf'&sb'&v&N1&N2).
+  exists sf' sb' v.
+  rewrite hstar_assoc, hstar_sep. splits~.
+Qed.
+
+Lemma triple_conseq : forall t H' Q' H Q,
+  triple t H' Q' ->
+  H ==> H' ->
+  Q' ===> Q ->
+  triple t H Q.
+Proof.
+  introv M N R.
+  unfolds triple.
+  intros Hf Hb. specializes M Hf Hb.
+  applys hoare_conseq.
+  applys M. applys~ himpl_frame_l.
+  intros v. applys~ himpl_frame_l.
+Qed.
+
+(*prove by hoare triple*)
+Lemma triple_conseq' : forall t H' Q' H Q,
+  triple t H' Q' ->
+  H ==> H' ->
+  Q' ===> Q ->
+  triple t H Q.
+Proof.
+  unfolds triple, hoare.
+  introv M MH MQ HF.
+  forwards (sf'&sb'&v&R&K): M sf sb. {applys~ himpl_frame_l MH HF. }
+  exists sf' sb' v. splits~. { applys~ himpl_frame_l. }
+Qed.
+
+Lemma triple_conseq_frame : forall H Q Hf Hb H1 Q1 t ,
+  triple t H1 Q1 ->
+  H ==> H1 \* (\R[Hf, Hb]) ->
+  Q1 \*+ (\R[Hf, Hb]) ===> Q ->
+  triple t H Q.
+Proof.
+  introv M N R.
+  unfolds triple.
+  intros Hf' Hb'.
+  specializes M (Hf \f* Hf') (Hb \b* Hb').
+  applys hoare_conseq. applys M.
+  rewrite <- hstar_sep, <- hstar_assoc;
+  applys~ himpl_frame_l.
+  intros v. rewrite <- hstar_sep. rewrite <- hstar_assoc.
+  applys~ himpl_frame_l.
+Qed.
+
+(*prove by hoare triple*)
+Lemma triple_conseq_frame' : forall H Q Hf Hb H1 Q1 t ,
+  triple t H1 Q1 ->
+  H ==> H1 \* (\R[Hf, Hb]) ->
+  Q1 \*+ (\R[Hf, Hb]) ===> Q ->
+  triple t H Q.
+Proof.
+  introv M N R.
+  unfolds triple, hoare.
+  intros Hf' Hb' sf sb ((sf1&sb1)&(sf2&sb2)&MA&MB&MC&MD).
+  forwards (sf'&sb'&v&T&K): M sf sb. rewrite MD.
+  lets K : himpl_frame_l (\R[Hf',Hb']) H (H1 \* (\R[Hf,Hb])).
+  rewrite hstar_assoc, hstar_sep in K.
+  apply K in N.  applys~ himpl_frame_l N. applys~ hstar_intro.
+  exists sf' sb' v. splits~.
+  applys~ himpl_frame_l. rewrite hstar_assoc, hstar_sep. auto.
+Qed.
+
+Lemma triple_ramified_frame : forall H1 t Hf Hb H Hf1 Hb1,
+  triple t H1 (fun r => \R[Hf1,Hb1]) ->
+  H ==> H1 \* (\R[Hf1 \f-* Hf, Hb1 \b-* Hb] ) ->
+  triple t H (fun r => \R[Hf,Hb]).
+Proof.
+  introv M W.
+  applys triple_conseq_frame M W.
+  intros v.
+  applys himpl_trans himpl_frame_r.
+  apply hwand_refine.
+  apply hwand_cancel.
+Qed.
+
+
+(*====== ramified_frame  ======*)
+(*Lemma triple_conseq_frame_of_ramified_frame : forall H2 H1 Hf1 Hb1 t H Hf Hb,
+  triple t H1 (fun r => \R[Hf1,Hb1]) ->
+  H ==> H1 \* H2 ->
+  (fun (r:val) => \R[Hf1,Hb1]) \*+ H2 ===> (fun r => \R[Hf,Hb]) ->
+  triple t H (fun r => \R[Hf,Hb]).
+Proof.
+  introv M WH WQ. applys triple_ramified_frame M.
+  applys himpl_trans WH.
+  applys himpl_frame_r.
+  applys himpl_trans.
+  rewrite qwand_equiv. applys WQ.
+Qed.*)
+
+
+(*---------- extract the prue fact and quantifier from precondition ----------*)
+Lemma triple_hpure : forall t (P:Prop) Hf Hb Q,
+  (P -> triple t (\R[Hf,Hb]) Q) ->
+  triple t (\[P] \* \R[Hf,Hb]) Q.
+Proof.
+  unfold triple. intros. rewrite hstar_assoc,hstar_sep.
+  intros hf hb M. apply hstar_hpure_iff in M as [MA MB].
+  applys~ H. rewrite~ hstar_sep.
+Qed.
+
+Lemma triple_hpure' : forall t (P:Prop) H Q,
+  (P -> triple t H Q) ->
+  triple t (\[P] \* H) Q.
+Proof.
+  unfold triple. intros. rewrite hstar_assoc.
+  intros hf hb M. apply hstar_hpure_iff in M as [MA MB].
+  applys~ H0.
+Qed.
+
+Lemma triple_hexists : forall t (A:Type) (J:A->hprop) Q,
+  (forall (x:A), triple t (J x) Q) ->
+  triple t (\exists (x:A), J x) Q.
+Proof.
+  unfold triple. intros.  intros hf hb M.
+  rewrite hstar_hexists in M.
+  destruct M as (v&M). specializes H v. applys~ H.
+Qed.
+
+Lemma triple_hbpure : forall t (P:Prop) Hf Hb Q,
+  (P -> triple t (\R[Hf,Hb]) Q) ->
+  triple t (\R[Hf,\b[P] \b* Hb]) Q.
+Proof.
+  unfold triple.
+  intros. intros hf hb. rewrite hstar_sep.
+  intros (MA&MB). simpls.
+  rewrite hbstar_assoc in MB.
+  apply hbstar_hpure_iff in MB as [MB1 MB2].
+  eapply H in MB1. apply MB1.
+  rewrite hstar_sep. splits~.
+Qed.
+
+Lemma triple_hfpure : forall t (P:Prop) Hf Hb Q,
+  (P -> triple t (\R[Hf,Hb]) Q) ->
+  triple t (\R[\f[P] \f* Hf,Hb]) Q.
+Proof.
+  unfold triple.
+  intros. intros hf hb. rewrite hstar_sep.
+  intros (MA&MB). simpls.
+  rewrite hfstar_assoc in MA.
+  apply hfstar_hpure_iff in MA as [MA1 MA2].
+  eapply H in MA1. apply MA1.
+  rewrite hstar_sep. splits~.
+Qed.
+
+Lemma triple_hbpure' : forall t (P:Prop) Hf Q,
+  (P -> triple t (\R[Hf,\b[]]) Q) ->
+  triple t (\R[Hf,\b[P]]) Q.
+Proof.
+  intros. lets M : triple_hbpure \b[].
+  rewrite~ hbstar_hempty_r in M.
+Qed.
+
+Lemma triple_hfpure' : forall t (P:Prop) Hb Q,
+  (P -> triple t (\R[\f[],Hb]) Q) ->
+  triple t (\R[\f[P],Hb]) Q.
+Proof.
+  intros. lets M : triple_hfpure \f[].
+  rewrite~ hfstar_hempty_r in M.
+Qed.
+
+Lemma triple_hbexists : forall t (A:Type) (J:A->hbprop) Hf Hb Q,
+  (forall (x:A), triple t (\R[ Hf, (J x) \b* Hb]) Q) ->
+  triple t (\R[ Hf, (\existsb (x:A), J x) \b* Hb]) Q.
+Proof.
+  unfold triple. intros. rewrite hstar_sep, hbstar_assoc.
+  intros hf hb (MA&MB). simpls.
+  rewrite hbstar_hexists in MB.
+  destruct MB as (v&MB).
+  specializes H v. apply H.
+  rewrite hstar_sep. splits~. rewrite~ hbstar_assoc.
+Qed.
+
+Lemma triple_hbexists' : forall t (A:Type) (J:A->hbprop) Hf Q,
+  (forall (x:A), triple t (\R[ Hf, (J x)]) Q) ->
+  triple t (\R[ Hf, (\existsb (x:A), J x)]) Q.
+Proof.
+  intros. lets M : triple_hbexists \b[].
+  rewrite~ hbstar_hempty_r in M. apply M.
+  intros. rewrite~ hbstar_hempty_r.
+Qed.
+
+Lemma triple_hfexists : forall t (A:Type) (J:A->hfprop) Hf Hb Q,
+  (forall (x:A), triple t (\R[(J x)\f*Hf, Hb]) Q) ->
+  triple t (\R[ (\existsf (x:A), J x) \f*Hf, Hb]) Q.
+Proof.
+  unfold triple. intros. rewrite hstar_sep, hfstar_assoc.
+  intros hf hb (MA&MB). simpls.
+  rewrite hfstar_hexists in MA.
+  destruct MA as (v&MA).
+  specializes H v. apply H.
+  rewrite hstar_sep. splits~. rewrite~ hfstar_assoc.
+Qed.
+
+Lemma triple_hfexists' : forall t (A:Type) (J:A->hfprop) Hb Q,
+  (forall (x:A), triple t (\R[ (J x), Hb]) Q) ->
+  triple t (\R[ (\existsf (x:A), J x), Hb]) Q.
+Proof.
+  intros. lets M : triple_hfexists \f[].
+  rewrite~ hfstar_hempty_r in M. apply M.
+  intros. rewrite~ hfstar_hempty_r.
+Qed.
+
+(*==================== AUX inner specification==============================*)
+Lemma hoare_bcreate' : forall Hf Hb ln,
+  hoare (bprim_create (val_listint ln))
+    (\R[ Hf, Hb])
+    (fun r => \R[ Hf, \existsb b, \b[r = val_bloc b] \b* b ~b~> ln \b* Hb ]).
+Proof.
+  intros. intros sf sb K0.
+  destruct K0 as (P1&P2).
+  forwards~ (b&D&N): (Fmap.single_fresh 0%nat sb ln).
+  exists sf ((Fmap.single b ln) \u sb) (val_bloc b). subst.
+  simpls. splits~.
+  (*Notice!!*)
+  - applys~ eval_bcreate_sep.
+  - splits~. exists b.
+    rewrite <- hbstar_assoc.
+    applys~ hbstar_intro.
+    rewrite~ hbstar_hpure. splits~.
+    applys~ hbsingle_intro.
+Qed.
+
+Lemma triple_bcreate' : forall Hf ln,
+  triple (bprim_create (val_listint ln))
+    (\R[ Hf, \b[] ])
+    (fun r => (\R[ Hf, (\existsb b, \b[r= (val_bloc b)] \b* b ~b~> ln)]) ).
+Proof.
+  intros. unfold triple. intros Hf' Hb'.
+  applys hoare_conseq hoare_bcreate' hstar_sep_l.
+
+  intros r h M.
+  destruct M as (MA&MB).
+  rewrite hstar_sep, state_get_eq.
+  splits~. simpls.
+  destruct MB as (pb&MB).
+  rewrite hbstar_hexists. exists pb.
+  apply hbstar_hpure_iff in MB as [MB1 MB].
+  rewrite hbstar_comm, hbstar_assoc, hbstar_hempty_l in MB.
+  rewrite~ hbstar_assoc. rewrite hbstar_hpure_iff.
+  splits~. rewrite~ hbstar_comm.
+Qed.
+
+(*====================== Optimization for Multi arguments =========================*)
+
+(*--- two arguments ---*)
+Lemma eval_like_app_fun2 : forall v0 v1 v2 x1 x2 t1,
+  v0 = val_fun x1 (trm_fun x2 t1) ->
+  (x1 <> x2) ->
+  eval_like (subst x2 v2 (subst x1 v1 t1)) (v0 v1 v2).
+Proof using.
+  introv E N. introv R.
+  applys~ eval_app_args.
+  - applys~ eval_app_fun E. simpl.
+    rewrite var_eq_spec. case_if.
+    applys eval_fun.
+  - applys eval_val.
+  - applys* eval_app_fun.
+Qed.
+
+Lemma eval_like_app_fix2 : forall F v0 v1 v2 x1 x2 t1,
+  v0 = val_fix F x1 (trm_fun x2 t1) ->
+  (x1 <> x2 /\ F <> x2) ->
+  eval_like (subst x2 v2 (subst x1 v1 (subst F v0 t1))) (v0 v1 v2).
+Proof using.
+  introv E (N1&N2). introv R.
+  applys~ eval_app_args.
+  - applys~ eval_app_fix E. simpl.
+    do 2 (rewrite var_eq_spec; case_if).
+    applys eval_fun.
+  - applys eval_val.
+  - applys* eval_app_fun.
+Qed.
+
+Lemma triple_app_fun2 : forall x1 x2 v0 v1 v2 t1 H Q,
+  v0 = val_fun x1 (trm_fun x2 t1) ->
+  (x1 <> x2) ->
+  triple (subst x2 v2 (subst x1 v1 t1)) H Q ->
+  triple (v0 v1 v2) H Q.
+Proof using.
+  introv E N M1. applys triple_eval_like M1. applys* eval_like_app_fun2.
+Qed.
+
+Lemma triple_app_fix2 : forall F x1 x2 v0 v1 v2 t1 H Q,
+  v0 = val_fix F x1 (trm_fun x2 t1) ->
+  (x1 <> x2 /\ F <> x2) ->
+  triple (subst x2 v2 (subst x1 v1 (subst F v0 t1))) H Q ->
+  triple (v0 v1 v2) H Q.
+Proof using.
+  introv E N M1. applys triple_eval_like M1. applys* eval_like_app_fix2.
+Qed.
+
+(* --- three args --- *)
+
+Lemma eval_like_app_fun3 : forall v0 v1 v2 v3 x1 x2 x3 t1,
+  v0 = val_fun x1 (trm_fun x2 (trm_fun x3 t1)) ->
+  (x1 <> x2  /\ x1 <> x3 /\ x2 <> x3) ->
+  eval_like (subst x3 v3 (subst x2 v2 (subst x1 v1 t1))) (v0 v1 v2 v3).
+Proof.
+  introv E (N1&N2&N3). introv R. applys* eval_app_args.
+  { applys* eval_like_app_fun2 E. simpl. do 2 (rewrite var_eq_spec; case_if). applys eval_fun. }
+  { applys eval_val. }
+  { applys* eval_app_fun. }
+Qed.
+
+Lemma triple_app_fun3 : forall x1 x2 x3 v0 v1 v2 v3 t1 H Q,
+  v0 = val_fun x1 (trm_fun x2 (trm_fun x3 t1)) ->
+  (x1 <> x2  /\ x1 <> x3 /\ x2 <> x3) ->
+  triple (subst x3 v3 (subst x2 v2 (subst x1 v1 t1))) H Q ->
+  triple (v0 v1 v2 v3) H Q.
+Proof.
+  introv E (N1&N2&N3) M.
+  applys triple_eval_like M. applys* eval_like_app_fun3.
+Qed.
+
+(*================== Reasoning rules for mapreduce ===========================*)
+(** ++++++++++++++++++++  Hoare Reasoning rules  ++++++++++++++++++++ **)
+
+(*------------ mapper opertions -------------------*)
+Lemma hoare_wdmap : forall Hf Hb b ln,
+  hoare (bMR_mapper (val_bloc b))
+    (\R[ Hf, ( (b ~b~> ln) \b* Hb) ])
+    ( fun r => \[r = (WCval_listwdpair (List.map init ln))] \* \R[ Hf, ((b ~b~> ln) \b* Hb)] ).
+Proof.
+  intros. intros sf sb K0.
+  destruct K0 as (P1&P2).
+  destruct P2 as (sb1&sb2&D1&D2&D3&D4).
+  exists sf sb (WCval_listwdpair (List.map init ln)). subst.
+  splits~.
+  - lets (E1&N) : hbsingle_inv D1. subst. simpls.
+    applys~ eval_wdmap_sep. apply D4.
+  - rewrite~ hstar_hpure. splits~. splits~. simpls. substs~.
+    applys~ hbstar_intro.
+Qed.
+
+(*-------- reducer --------*)
+
+Lemma hoare_wdmerge : forall H Lwd,
+  hoare (fMR_merge (WCval_Listwd Lwd)) H
+    (fun r => (\[r = WCval_listwdpair (fold_right app nil Lwd)] \* H)).
+Proof.
+  intros. intros sf sb.
+  intros M.
+  exists sf sb (WCval_listwdpair (fold_right app nil Lwd)). splits.
+  apply eval_merge.
+  applys* hstar_hpure_iff.
+Qed.
+
+Lemma hoare_wdreduce : forall H Lwd,
+  hoare (fMR_reducer (WCval_Listwd Lwd)) H
+    (fun r => (\[r = WCval_listwdpair (List.map accmulate Lwd)] \* H)).
+Proof.
+  intros. intros sf sb.
+  intros M.
+  exists sf sb (WCval_listwdpair (List.map accmulate Lwd)). splits.
+  apply eval_wdreduce.
+  applys* hstar_hpure_iff.
+Qed.
+(*------------------ SL rule: mapper ---------------*)
+
+(** WordCount mapper rules **)
+Lemma triple_wdmap : forall Hf b ln,
+  triple (bMR_mapper (val_bloc b))
+    (\R[ Hf, (b ~b~> ln) ])
+    ( fun r => \[r = (WCval_listwdpair (List.map init ln))] \* \R[ Hf, (b ~b~> ln)] ).
+Proof.
+  intros. unfold triple. intros Hf' Hb'.
+  applys hoare_conseq hoare_wdmap.
+  rewrite hstar_sep. apply himpl_refl.
+  intros r h R.
+  rewrite hstar_hpure_iff in R.
+  destruct R as (RA&RB).
+  rewrite hstar_assoc. rewrite hstar_hpure.
+  splits~. rewrite~ hstar_sep.
+Qed.
+
+(*------------------ SL rule: reducer ---------------*)
+
+(** WordCount reducer rules **)
+Lemma triple_wdmerge : forall H Lwd,
+  triple (fMR_merge (WCval_Listwd Lwd)) H
+    (fun r => (\[r = WCval_listwdpair (fold_right app nil Lwd)] \* H)).
+Proof.
+  intros. intros Hf Hb sf sb M.
+  exists sf sb (WCval_listwdpair (fold_right app nil Lwd)). splits.
+  apply eval_merge. rewrite hstar_assoc.
+  applys* hstar_hpure_iff.
+Qed.
+
+Lemma triple_wdgroup : forall H lwd,
+  triple (fMR_group (WCval_listwdpair lwd)) H
+    (fun r => (\[r = WCval_Listwd (remove_duplicates (classify lwd lwd))] \* H)).
+Proof.
+  intros. intros Hf Hb sf sb M.
+  exists sf sb (WCval_Listwd (remove_duplicates (classify lwd lwd))). splits.
+  apply eval_group. rewrite hstar_assoc.
+  applys* hstar_hpure_iff.
+Qed.
+
+Lemma triple_wdreduce : forall H Lwd,
+  triple (fMR_reducer (WCval_Listwd Lwd)) H
+    (fun r => (\[r = WCval_listwdpair (List.map accmulate Lwd)] \* H)).
+Proof.
+  intros. intros Hf Hb sf sb M.
+  exists sf sb (WCval_listwdpair (List.map accmulate Lwd)). splits.
+  apply eval_wdreduce. rewrite hstar_assoc.
+  applys* hstar_hpure_iff.
+Qed.
+
+(* rules for aux list operations *)
+Lemma triple_app_wdlist : forall H l L,
+  triple (val_app_wdlist (WCval_listwdpair l) (WCval_Listwd L)) H
+    (fun r => (\[r = WCval_Listwd (l :: L)] \* H)).
+Proof.
+  intros. intros Hf Hb sf sb M.
+  exists sf sb (WCval_Listwd (l :: L)). splits.
+  apply eval_app_wdlist. rewrite hstar_assoc.
+  applys* hstar_hpure_iff.
+Qed.
+
+Lemma triple_MRlist_reform : forall H l1,
+  triple (val_reform (WCval_listwdpair l1)) H
+    (fun r => (\[r = val_listint (kv2int l1)] \* H)).
+Proof.
+  intros. unfold triple. intros Hf Hb sf sb M.
+  exists sf sb (val_listint (kv2int l1)).
+  splits~. apply eval_reform.
+  rewrite hstar_assoc.
+  apply* hstar_hpure_iff.
+Qed.
+
+(* ================================================================================ *)
