Readme.md
@@ -1,44 +1,48 @@
-# Formal Verification for Cloud Block Storage in Coq
+# Formal Verification of Cloud Block Storage in Coq
 
 To rigorously discuss the reliability of cloud block storage (CBS), we develop a proof system and implement a verification tool for reasoning about the correctness of CBS data operations. The proof system has separation logic features, and the tool simplifies derivation while retaining mathematical rigor.
 
-This proof system consists of the modeling language, heap predicates, triples, and reasoning rules. The modeling language represents CBS state and data operations, and the heap predicates describe the properties of a given CBS state. Besides, the triples specify the behavior of a program, and the reasoning rules supports verifying these triples.
+This proof system consists of the modeling language, heap predicates, triples, and reasoning rules. The modeling language represents CBS state and data operations, and the heap predicates describe the properties of a given CBS state. Besides, the triples specify the correct behavior of a program, and the reasoning rules supports verifying those triples.
 
-We implement this proof system as a verification tool in Coq. Our tool can encode actual operations intuitively and verify specifications semi-automatically. The notations and type conversions in our tool improve the readability of the representation code. The automated proof scripts simplify the verifying process and skip the unnecessary details. 
-
-In particular, the data modifications in CBS are more likely to cause logical storage errors, such as null reference or block loss. Therefore, in addition to the basic operations, we represent and verify the CBS data modifications to thus analyze their mathematical correctness.
+We implement this proof system as a verification tool in Coq. Our tool can encode actual operations intuitively and verify specifications efficiently. The notations and type conversions in our tool improve the readability of the representation code. The automated proof scripts simplify the verifying process and skip the unnecessary details. 
 
 ## How We Reason about CBS Programs
 
 First, code a function with the modeling language to represent an actual CBS data operation.
 
 ```Coq
-Definition Copy_blk : val := 
-  Fun bk :=
-    Let ln := bget bk in    (* read the content of a block *)
-      bcreate ln.           (* create a block *)
+Definition CopyBlk : val := 
+  Fun 'f 'n := 
+  	Let 'b := 'nthblk 'f 'n in     (* get the target block's loction *)
+    Let 'ln := 'bget 'b in         (* get the block's contents *)
+      'bcreate 'ln                 (* create a new block *)
 ```
 
 Second, specify the invocation of this function by a triple. This triple captures the system properties before and after the function invocation.
 
 ```Coq
-Lemma triple_Copy_blk : forall (Hf:hfprop) (bp:bloc) (ln:listint),
-  triple (Copy_blk bp)
-    (\R[Hf, bp~b~>ln])
-    (fun r => \exists bp', [r=bp'] \* \R[Hf,((bp'~b~>ln) \b* (bp~b~>ln))]).
+Lemma triple_CopyBlk : forall (f:floc) (b:bloc) (lb:list bloc) (ln:list int) (n:int),
+  triple (CopyBlk f n)  (* invocate the function *)
+(* pre-condition: the pure fact constrains the location; the predicate describes the storage of the target block *)
+    ( \[b = nth n lb] \* \R[f ~f~> lb, b ~b~> ln] )
+(* post-condition: the pure fact describes the new block's location; the predicate additionally declares that a new block has been created *) 
+    ( fun r => \exists (b1:bloc), \[r=b1] \* (\R[f ~f~> lb,(b1 ~b~> ln) \b* (b ~b~> ln)]) ).
 ```
 
 Last, reason and prove such a triple using the proven reasoning rules. If this triple can be proved, it is sound since the reasoning rules are all sound. 
 
 ```Coq
 Proof.
-  intros. applys* triple_app_fun.             (* reason about invoking a funcation *)
-  applys triple_let triple_bget. ext.         (* reason about reading a block *)
-  applys triple_conseq_frame triple_bcreate.  (* reason about creating a new block *)
-  rewrite* hstar_hempty_l'.                   (* rewrite the format and complete proof *)
+  intros. apply triple_hpure. intros ->.
+  applys* triple_app_fun2. ext.                (* invoke a funcation *)
+  applys* triple_let triple_fget_nth_blk. ext. (* get the block's loc *)
+  applys triple_let triple_bget. ext.          (* get the block's contents *)
+  applys triple_conseq_frame triple_bcreate.   (* create a new block *)
+  rewrite* hstar_hempty_l'.                  (* rewrite the format and complete proof *)
   introv M. rewrite hstar_hexists in M.
-  destruct M as (bp'&M). rewrite hstar_assoc, hstar_sep, hfstar_hempty_l in M.
-  exists~ bp'.
+  destruct M as (b1&M).
+  rewrite hstar_assoc, hstar_sep, hfstar_hempty_l in M.
+  exists~ b1.
 Qed.
 ```
 
@@ -47,15 +51,25 @@ Qed.
 The Implementation of our proof system mainly consists the following parts:.
 
 - Modeling Language  ——  Language.v
-- Assertion Language  ——  CBS heap predicates (Himpl.v) + Internal heap predicates (InnerPre.v) 
-- Specification Language  ——  Rules.v
-- Verification of Basic Operations  ——  ExBasic.v
-- Verification of Data Modifications ——  Example.v
+- Assertion Language  ——  CBS heap predicates (Himpl.v) + Internal heap predicates (InnerPre.v)
+- Hoare Logic  —— Hoare.v
+- The proof system for CBS —— TripleAndRules.v
+- Verification of basic operations  ——  ExBasic.v
+- Verification of data modifications ——  ExModification.v
+- Verification of a MapReduce application (WordCount) ——  ExMapReduce.v
 - Variable Notations —— Var.v 
 
 In additions, our tool depends on a Coq standard library (TLC.v) and a definition of finite map (Fmap.v).
 
-The implementation of the verification tool amount to 4601 non-blank lines of Coq script. It includes 80 definitions, 313 lemmas, and the verifications of 8 scenarios.
+The implementation of the verification tool amount to 5664 non-blank lines of Coq script. It includes 115 definitions, 368 lemmas, and the verifications of 12 scenarios.
+
+## Environment
+
+- Coq Version : Coq 8.8.0
+
+- IDE : VScode
+
+- OS : Windows 10
 
 ## Installation
 
@@ -69,11 +83,11 @@ To install the latest development version of our tool, use this:
   make
 ```
 
-**Note** : No Chinese is allowed in the file path!
+**Note** : <font color=red>No Chinese is allowed in the file path!</font>
 
 ## Replaying a sample proof
 
-Then, you can load an example proof. There are several examples in the file Example.v. Just use the CoqIDE to open that file and check the proof. The success proof of a program will be as follows.
+Then, you can load an example proof. There are several examples in the files ExBasic.v, ExModification.v, and ExMapReduce.v. Just use the CoqIDE to open a file and check the corresponding proof. The success proof of a program will be as follows.
 
-<img src="Move.png" alt="avatar" style="zoom:30%;" />
+<img src="Move.png" alt="avatar" style="zoom:50%;" />
 
